@prefix activities: <http://purl.org/procurement/public-contracts-activities#> .
@prefix adms: <http://www.w3.org/ns/adms#> .
@prefix authkinds: <http://purl.org/procurement/public-contracts-authority-kinds#> .
@prefix c4n: <http://vocab.deri.ie/c4n#> .
@prefix criteria: <http://purl.org/procurement/public-contracts-criteria#> .
@prefix dc: <http://purl.org/dc/elements/1.1/> .
@prefix dcterms: <http://purl.org/dc/terms/> .
@prefix foaf: <http://xmlns.com/foaf/0.1/> .
@prefix gn: <http://www.geonames.org/ontology#> .
@prefix gr: <http://purl.org/goodrelations/v1#> .
@prefix kinds: <http://purl.org/procurement/public-contracts-kinds#> .
@prefix loted: <http://www.loted.eu/ontology#> .
@prefix owl: <http://www.w3.org/2002/07/owl#> .
@prefix payment: <http://reference.data.gov.uk/def/payment#> .
@prefix pc: <http://purl.org/procurement/public-contracts#> .
@prefix pcdt: <http://purl.org/procurement/public-contracts-datatypes#> .
@prefix proctypes: <http://purl.org/procurement/public-contracts-procedure-types#> .
@prefix qb: <http://purl.org/linked-data/cube#> .
@prefix rdf: <http://www.w3.org/1999/02/22-rdf-syntax-ns#> .
@prefix rdfs: <http://www.w3.org/2000/01/rdf-schema#> .
@prefix schema: <http://schema.org/> .
@prefix skos: <http://www.w3.org/2004/02/skos/core#> .
@prefix vann: <http://purl.org/vocab/vann/> .
@prefix wgs: <http://www.w3.org/2003/01/geo/wgs84_pos#> .
@prefix xsd: <http://www.w3.org/2001/XMLSchema#> .

<http://purl.org/procurement/public-contracts> a owl:Ontology .

<http://purl.org/klimek#me> a foaf:Person .

<http://purl.org/knap#me> a foaf:Person .

<http://www.ksi.mff.cuni.cz/~necasky> a foaf:Person .

<http://www.facebook.com/nohis> a foaf:Person .

<http://keg.vse.cz/resource/person/josef-petrak> a foaf:Person .

<http://keg.vse.cz/resource/person/vojtech-svatek> a foaf:Person .

<http://keg.vse.cz/resource/person/jindrich-mynarz> a foaf:Person .

pc:Contract a owl:Class .

pc:FrameworkAgreement a owl:Class .

pc:Tender a owl:Class .

gr:Offering a owl:Class .

pc:AwardCriteriaCombination a owl:Class .

pc:CriterionWeighting a owl:Class .

pc:TendersOpening a owl:Class .

pc:awardDate a owl:DatatypeProperty, owl:FunctionalProperty .

pc:contact a owl:FunctionalProperty, owl:ObjectProperty .

pc:kind a qb:CodedProperty, owl:FunctionalProperty, owl:ObjectProperty .

pc:procedureType a qb:CodedProperty, owl:FunctionalProperty, owl:ObjectProperty .

pc:contractingAuthority a owl:FunctionalProperty, owl:ObjectProperty .

gr:BusinessEntity a owl:Class .

pc:item a owl:ObjectProperty .

pc:mainObject a owl:FunctionalProperty, owl:ObjectProperty .

pc:additionalObject a owl:ObjectProperty .

pc:location a owl:ObjectProperty .

schema:Place a owl:Class .

pc:contractPrice a owl:ObjectProperty .

gr:PriceSpecification a owl:Class .

pc:documentationPrice a owl:FunctionalProperty, owl:ObjectProperty .

pc:estimatedPrice a owl:FunctionalProperty, owl:ObjectProperty .

pc:tenderDeadline a owl:DatatypeProperty, owl:FunctionalProperty .

pc:documentationRequestDeadline a owl:DatatypeProperty, owl:FunctionalProperty .

pc:duration a owl:DatatypeProperty, owl:FunctionalProperty .

pc:tenderMaintenanceDuration a owl:DatatypeProperty, owl:FunctionalProperty .

pc:startDate a owl:DatatypeProperty, owl:FunctionalProperty .

pc:estimatedEndDate a owl:DatatypeProperty, owl:FunctionalProperty .

pc:actualEndDate a owl:DatatypeProperty, owl:FunctionalProperty .

pc:awardCriteriaCombination a owl:FunctionalProperty, owl:ObjectProperty .

pc:lot a owl:ObjectProperty .

pc:frameworkAgreement a owl:ObjectProperty .

pc:numberOfTenders a owl:DatatypeProperty, owl:FunctionalProperty .

pc:tender a owl:ObjectProperty .

pc:awardedTender a owl:FunctionalProperty, owl:ObjectProperty .

pc:subsidy a owl:ObjectProperty .

pc:agreedPrice a owl:FunctionalProperty, owl:ObjectProperty .

pc:actualPrice a owl:FunctionalProperty, owl:ObjectProperty .

pc:attachment a owl:ObjectProperty .

pc:specification a owl:ObjectProperty .

pc:agreement a owl:ObjectProperty .

pc:awardCriterion a owl:ObjectProperty .

pc:expectedNumberOfOperators a owl:FunctionalProperty, owl:ObjectProperty .

gr:QuantitativeValueInteger a owl:Class .

pc:profile a owl:DatatypeProperty .

pc:authorityKind a qb:CodedProperty, owl:FunctionalProperty, owl:ObjectProperty .

pc:mainActivity a qb:CodedProperty, owl:FunctionalProperty, owl:ObjectProperty .

pc:offeredPrice a owl:FunctionalProperty, owl:ObjectProperty .

gr:hasPriceSpecification a owl:ObjectProperty .

pc:bidder a owl:ObjectProperty .

pc:contract a owl:ObjectProperty .

pc:weightedCriterion a owl:FunctionalProperty, owl:ObjectProperty .

pc:criterionWeight a owl:DatatypeProperty, owl:FunctionalProperty .

gr:availabilityStarts a owl:DatatypeProperty .

schema:Offer a owl:Class .

<http://purl.org/goodrelations/v1> a owl:Ontology .

dc:title a owl:AnnotationProperty .

dc:subject a owl:AnnotationProperty .

dc:creator a owl:AnnotationProperty .

dc:rights a owl:AnnotationProperty .

dcterms:license a owl:AnnotationProperty .

dc:contributor a owl:AnnotationProperty .

foaf:homepage a owl:AnnotationProperty .

gr:availableAtOrFrom a owl:ObjectProperty .

gr:Location a owl:Class .

gr:taxID a owl:DatatypeProperty .

schema:Organization a owl:Class .

schema:Person a owl:Class .

gr:seeks a owl:ObjectProperty .

gr:Reseller a gr:BusinessEntityType .

gr:BusinessEntityType a owl:Class .

gr:amountOfThisGood a owl:DatatypeProperty .

gr:TypeAndQuantityNode a owl:Class .

gr:serialNumber a owl:DatatypeProperty .

gr:Individual a owl:Class .

schema:Product a owl:Class .

gr:hasISICv4 a owl:DatatypeProperty .

gr:opens a owl:DatatypeProperty .

gr:OpeningHoursSpecification a owl:Class .

gr:hasNAICS a owl:DatatypeProperty .

gr:legalName a owl:DatatypeProperty .

gr:FederalExpress a gr:DeliveryModeParcelService .

gr:DeliveryModeParcelService a owl:Class .

gr:hasMPN a owl:DatatypeProperty .

schema:productID a owl:DatatypeProperty .

gr:ProductOrService a owl:Class .

gr:vatID a owl:DatatypeProperty .

gr:DHL a gr:DeliveryModeParcelService .

gr:DeliveryModeMail a gr:DeliveryMethod .

gr:DeliveryMethod a owl:Class .

gr:category a owl:DatatypeProperty .

gr:hasPOS a owl:ObjectProperty .

gr:availabilityEnds a owl:DatatypeProperty .

gr:eligibleCustomerTypes a owl:ObjectProperty .

gr:ByInvoice a gr:PaymentMethod .

gr:PaymentMethod a owl:Class .

gr:hasInventoryLevel a owl:ObjectProperty .

gr:QuantitativeValueFloat a owl:Class .

gr:SomeItems a owl:Class .

gr:isSimilarTo a owl:ObjectProperty .

gr:Maintain a gr:BusinessFunction .

gr:BusinessFunction a owl:Class .

gr:hasOpeningHoursSpecification a owl:ObjectProperty .

gr:validThrough a owl:DatatypeProperty .

gr:License a owl:Class .

gr:AmericanExpress a gr:PaymentMethodCreditCard .

gr:PaymentMethodCreditCard a owl:Class .

gr:appliesToPaymentMethod a owl:ObjectProperty .

gr:PaymentChargeSpecification a owl:Class .

gr:isConsumableFor a owl:ObjectProperty .

gr:hasValueFloat a owl:DatatypeProperty .

gr:hasMaxValueFloat a owl:DatatypeProperty .

gr:hasMaxValue a owl:DatatypeProperty .

gr:hasMinValueFloat a owl:DatatypeProperty .

gr:hasMinValue a owl:DatatypeProperty .

gr:closes a owl:DatatypeProperty .

gr:PaySwarm a gr:PaymentMethod .

gr:advanceBookingRequirement a owl:ObjectProperty .

gr:eligibleTransactionVolume a owl:ObjectProperty .

gr:durationOfWarrantyInMonths a owl:DatatypeProperty .

gr:WarrantyPromise a owl:Class .

gr:hasGlobalLocationNumber a owl:DatatypeProperty .

gr:isVariantOf a owl:ObjectProperty .

gr:ProductOrServiceModel a owl:Class .

gr:hasGTIN-8 a owl:DatatypeProperty .

gr:PartsAndLabor-PickUp a gr:WarrantyScope .

gr:WarrantyScope a owl:Class .

gr:JCB a gr:PaymentMethodCreditCard .

gr:depth a owl:ObjectProperty .

gr:QuantitativeValue a owl:Class .

gr:quantitativeProductOrServiceProperty a owl:ObjectProperty .

gr:hasValueInteger a owl:DatatypeProperty .

gr:hasMinValueInteger a owl:DatatypeProperty .

gr:hasMaxValueInteger a owl:DatatypeProperty .

schema:manufacturer a owl:ObjectProperty .

gr:hasManufacturer a owl:ObjectProperty .

schema:description a owl:DatatypeProperty .

gr:description a owl:DatatypeProperty .

gr:Brand a owl:Class .

gr:DayOfWeek a owl:Class .

gr:DeliveryChargeSpecification a owl:Class .

gr:QualitativeValue a owl:Class .

gr:UnitPriceSpecification a owl:Class .

gr:Cash a gr:PaymentMethod .

gr:DinersClub a gr:PaymentMethodCreditCard .

gr:Dispose a gr:BusinessFunction .

gr:billingIncrement a owl:DatatypeProperty .

gr:isListPrice a owl:DatatypeProperty .

owl:deprecated a owl:AnnotationProperty .

gr:color a owl:DatatypeProperty .

gr:datatypeProductOrServiceProperty a owl:DatatypeProperty .

gr:isAccessoryOrSparePartFor a owl:ObjectProperty .

gr:hasDUNS a owl:DatatypeProperty .

gr:typeOfGood a owl:ObjectProperty .

gr:deliveryLeadTime a owl:ObjectProperty .

gr:hasStockKeepingUnit a owl:DatatypeProperty .

gr:qualitativeProductOrServiceProperty a owl:ObjectProperty .

gr:availableDeliveryMethods a owl:ObjectProperty .

gr:Repair a gr:BusinessFunction .

gr:GoogleCheckout a gr:PaymentMethod .

gr:includes a owl:ObjectProperty .

gr:Business a gr:BusinessEntityType .

gr:Sell a gr:BusinessFunction .

gr:hasValue a owl:DatatypeProperty .

gr:hasBrand a owl:ObjectProperty .

gr:ByBankTransferInAdvance a gr:PaymentMethod .

gr:hasOpeningHoursDayOfWeek a owl:ObjectProperty .

gr:priceType a owl:DatatypeProperty .

gr:DeliveryModeOwnFleet a gr:DeliveryMethod .

gr:eligibleRegions a owl:DatatypeProperty .

gr:VISA a gr:PaymentMethodCreditCard .

gr:valueReference a owl:ObjectProperty .

gr:validFrom a owl:DatatypeProperty .

gr:DeliveryModeDirectDownload a gr:DeliveryMethod .

gr:UPS a gr:DeliveryModeParcelService .

gr:ConstructionInstallation a gr:BusinessFunction .

gr:CheckInAdvance a gr:PaymentMethod .

schema:name a owl:DatatypeProperty .

gr:name a owl:DatatypeProperty .

gr:hasWarrantyPromise a owl:ObjectProperty .

gr:hasGTIN-14 a owl:DatatypeProperty .

gr:LeaseOut a gr:BusinessFunction .

gr:hasCurrencyValue a owl:DatatypeProperty .

gr:hasMinCurrencyValue a owl:DatatypeProperty .

gr:hasMaxCurrencyValue a owl:DatatypeProperty .

gr:hasCurrency a owl:DatatypeProperty .

gr:Buy a gr:BusinessFunction .

gr:hasMakeAndModel a owl:ObjectProperty .

gr:PartsAndLabor-BringIn a gr:WarrantyScope .

gr:Enduser a gr:BusinessEntityType .

gr:relatedWebService a owl:AnnotationProperty .

gr:PublicHolidays a gr:DayOfWeek .

gr:displayPosition a owl:AnnotationProperty .

gr:valueAddedTaxIncluded a owl:DatatypeProperty .

gr:acceptedPaymentMethods a owl:ObjectProperty .

gr:hasBusinessFunction a owl:ObjectProperty .

gr:hasWarrantyScope a owl:ObjectProperty .

gr:weight a owl:ObjectProperty .

gr:includesObject a owl:ObjectProperty .

gr:hasEAN_UCC-13 a owl:DatatypeProperty .

gr:N-Ary-Relations a owl:Class .

gr:equal a owl:ObjectProperty, owl:SymmetricProperty, owl:TransitiveProperty .

gr:Labor-BringIn a gr:WarrantyScope .

gr:height a owl:ObjectProperty .

gr:width a owl:ObjectProperty .

gr:COD a gr:PaymentMethod .

gr:hasEligibleQuantity a owl:ObjectProperty .

schema:image a owl:ObjectProperty .

foaf:depiction a owl:ObjectProperty .

gr:DeliveryModeFreight a gr:DeliveryMethod .

gr:eligibleDuration a owl:ObjectProperty .

gr:PayPal a gr:PaymentMethod .

gr:nonEqual a owl:ObjectProperty, owl:SymmetricProperty .

gr:condition a owl:DatatypeProperty .

gr:PublicInstitution a gr:BusinessEntityType .

gr:DeliveryModePickUp a gr:DeliveryMethod .

gr:Discover a gr:PaymentMethodCreditCard .

gr:DirectDebit a gr:PaymentMethod .

gr:ProvideService a gr:BusinessFunction .

gr:appliesToDeliveryMethod a owl:ObjectProperty .

gr:owns a owl:ObjectProperty .

gr:MasterCard a gr:PaymentMethodCreditCard .

gr:hasUnitOfMeasurement a owl:DatatypeProperty .

gr:offers a owl:ObjectProperty .

gr:addOn a owl:ObjectProperty .

gr:Wednesday a gr:DayOfWeek .

gr:hasNext a owl:ObjectProperty .

gr:Thursday a gr:DayOfWeek .

gr:Friday a gr:DayOfWeek .

gr:hasPrevious a owl:ObjectProperty .

gr:Tuesday a gr:DayOfWeek .

gr:Monday a gr:DayOfWeek .

gr:lesser a owl:ObjectProperty, owl:TransitiveProperty .

gr:greater a owl:ObjectProperty, owl:TransitiveProperty .

gr:LocationOfSalesOrServiceProvisioning a owl:Class .

gr:ProductOrServicesSomeInstancesPlaceholder a owl:Class .

gr:predecessorOf a owl:ObjectProperty, owl:TransitiveProperty .

gr:successorOf a owl:ObjectProperty, owl:TransitiveProperty .

gr:Sunday a gr:DayOfWeek .

gr:Saturday a gr:DayOfWeek .

gr:ActualProductOrServiceInstance a owl:Class .

gr:greaterOrEqual a owl:ObjectProperty, owl:TransitiveProperty .

gr:lesserOrEqual a owl:ObjectProperty, owl:TransitiveProperty .

pc:awardDate rdfs:subPropertyOf dcterms:date .

pc:kind rdfs:subPropertyOf dcterms:type .

pc:item rdfs:subPropertyOf dcterms:hasPart .

pc:mainObject rdfs:subPropertyOf dcterms:subject .

pc:additionalObject rdfs:subPropertyOf dcterms:subject .

pc:location rdfs:subPropertyOf schema:location .

pc:estimatedPrice rdfs:subPropertyOf pc:contractPrice .

pc:tenderDeadline rdfs:subPropertyOf dcterms:date .

pc:documentationRequestDeadline rdfs:subPropertyOf dcterms:date .

pc:startDate rdfs:subPropertyOf dcterms:date .

pc:estimatedEndDate rdfs:subPropertyOf dcterms:date .

pc:actualEndDate rdfs:subPropertyOf dcterms:date .

pc:awardedTender rdfs:subPropertyOf pc:tender .

pc:agreedPrice rdfs:subPropertyOf pc:contractPrice .

pc:actualPrice rdfs:subPropertyOf pc:contractPrice .

pc:specification rdfs:subPropertyOf pc:attachment .

pc:agreement rdfs:subPropertyOf pc:attachment .

pc:offeredPrice rdfs:subPropertyOf gr:hasPriceSpecification .

pc:weightedCriterion rdfs:subPropertyOf dcterms:subject .

gr:hasMPN rdfs:subPropertyOf schema:productID .

gr:hasValueFloat rdfs:subPropertyOf gr:hasMaxValueFloat, gr:hasMinValueFloat .

gr:hasMaxValueFloat rdfs:subPropertyOf gr:hasMaxValue .

gr:hasMinValueFloat rdfs:subPropertyOf gr:hasMinValue .

gr:hasGTIN-8 rdfs:subPropertyOf schema:productID .

gr:depth rdfs:subPropertyOf gr:quantitativeProductOrServiceProperty .

gr:hasValueInteger rdfs:subPropertyOf gr:hasMaxValueInteger, gr:hasMinValueInteger .

gr:hasMinValueInteger rdfs:subPropertyOf gr:hasMinValue .

gr:hasMaxValueInteger rdfs:subPropertyOf gr:hasMaxValue .

gr:color rdfs:subPropertyOf gr:datatypeProductOrServiceProperty .

gr:hasStockKeepingUnit rdfs:subPropertyOf schema:productID .

gr:hasValue rdfs:subPropertyOf gr:hasMaxValue, gr:hasMinValue .

gr:hasGTIN-14 rdfs:subPropertyOf schema:productID .

gr:hasCurrencyValue rdfs:subPropertyOf gr:hasMaxCurrencyValue, gr:hasMinCurrencyValue .

gr:weight rdfs:subPropertyOf gr:quantitativeProductOrServiceProperty .

gr:hasEAN_UCC-13 rdfs:subPropertyOf schema:productID .

gr:height rdfs:subPropertyOf gr:quantitativeProductOrServiceProperty .

gr:width rdfs:subPropertyOf gr:quantitativeProductOrServiceProperty .

pc:Tender rdfs:subClassOf gr:Offering .

pc:CriterionWeighting rdfs:subClassOf c4n:Condition .

pc:TendersOpening rdfs:subClassOf schema:Event .

gr:QuantitativeValueInteger rdfs:subClassOf gr:QuantitativeValue .

schema:Offer rdfs:subClassOf gr:Offering .

schema:Organization rdfs:subClassOf gr:BusinessEntity .

schema:Person rdfs:subClassOf gr:BusinessEntity .

gr:Individual rdfs:subClassOf gr:ProductOrService, schema:Product .

gr:DeliveryModeParcelService rdfs:subClassOf gr:DeliveryMethod .

gr:QuantitativeValueFloat rdfs:subClassOf gr:QuantitativeValue .

gr:SomeItems rdfs:subClassOf gr:ProductOrService, schema:Product .

gr:License rdfs:subClassOf gr:BusinessFunction .

gr:PaymentMethodCreditCard rdfs:subClassOf gr:PaymentMethod .

gr:PaymentChargeSpecification rdfs:subClassOf gr:PriceSpecification .

gr:ProductOrServiceModel rdfs:subClassOf gr:ProductOrService, schema:Product .

gr:DeliveryChargeSpecification rdfs:subClassOf gr:PriceSpecification .

gr:UnitPriceSpecification rdfs:subClassOf gr:PriceSpecification .

gr:ProductOrServicesSomeInstancesPlaceholder rdfs:subClassOf gr:ProductOrService .

gr:ActualProductOrServiceInstance rdfs:subClassOf gr:ProductOrService .

pc:awardDate rdfs:domain pc:Contract .

pc:contact rdfs:domain pc:Contract .

pc:kind rdfs:domain pc:Contract .

pc:procedureType rdfs:domain pc:Contract .

pc:contractingAuthority rdfs:domain pc:Contract .

pc:item rdfs:domain _:node3 .

_:node3 a owl:Class .

pc:mainObject rdfs:domain pc:Contract .

pc:additionalObject rdfs:domain pc:Contract .

pc:location rdfs:domain pc:Contract .

pc:contractPrice rdfs:domain pc:Contract .

pc:documentationPrice rdfs:domain pc:Contract .

pc:tenderDeadline rdfs:domain pc:Contract .

pc:documentationRequestDeadline rdfs:domain pc:Contract .

pc:duration rdfs:domain pc:Contract .

pc:tenderMaintenanceDuration rdfs:domain pc:Contract .

pc:startDate rdfs:domain pc:Contract .

pc:estimatedEndDate rdfs:domain pc:Contract .

pc:actualEndDate rdfs:domain pc:Contract .

pc:awardCriteriaCombination rdfs:domain pc:Contract .

pc:lot rdfs:domain pc:Contract .

pc:frameworkAgreement rdfs:domain pc:Contract .

pc:numberOfTenders rdfs:domain pc:Contract .

pc:tender rdfs:domain pc:Contract .

pc:subsidy rdfs:domain pc:Contract .

pc:attachment rdfs:domain pc:Contract .

pc:awardCriterion rdfs:domain pc:AwardCriteriaCombination .

pc:expectedNumberOfOperators rdfs:domain pc:FrameworkAgreement .

pc:profile rdfs:domain gr:BusinessEntity .

pc:authorityKind rdfs:domain gr:BusinessEntity .

pc:mainActivity rdfs:domain gr:BusinessEntity .

pc:offeredPrice rdfs:domain pc:Tender .

gr:hasPriceSpecification rdfs:domain _:node98 .

_:node98 a owl:Class .

pc:bidder rdfs:domain pc:Tender .

pc:contract rdfs:domain pc:TendersOpening .

pc:weightedCriterion rdfs:domain pc:CriterionWeighting .

pc:criterionWeight rdfs:domain pc:CriterionWeighting .

gr:availabilityStarts rdfs:domain _:node8 .

_:node8 a owl:Class .

gr:availableAtOrFrom rdfs:domain _:node11 .

_:node11 a owl:Class .

gr:taxID rdfs:domain _:node14 .

_:node14 a owl:Class .

gr:seeks rdfs:domain _:node18 .

_:node18 a owl:Class .

gr:amountOfThisGood rdfs:domain gr:TypeAndQuantityNode .

gr:serialNumber rdfs:domain _:node22 .

_:node22 a owl:Class .

gr:hasISICv4 rdfs:domain _:node26 .

_:node26 a owl:Class .

gr:opens rdfs:domain gr:OpeningHoursSpecification .

gr:hasNAICS rdfs:domain _:node31 .

_:node31 a owl:Class .

gr:legalName rdfs:domain _:node34 .

_:node34 a owl:Class .

gr:hasMPN rdfs:domain _:node37 .

_:node37 a owl:Class .

gr:vatID rdfs:domain _:node41 .

_:node41 a owl:Class .

gr:category rdfs:domain _:node45 .

_:node45 a owl:Class .

gr:hasPOS rdfs:domain _:node54 .

_:node54 a owl:Class .

gr:availabilityEnds rdfs:domain _:node57 .

_:node57 a owl:Class .

gr:eligibleCustomerTypes rdfs:domain _:node60 .

_:node60 a owl:Class .

gr:hasInventoryLevel rdfs:domain _:node63 .

_:node63 a owl:Class .

gr:isSimilarTo rdfs:domain _:node67 .

_:node67 a owl:Class .

gr:hasOpeningHoursSpecification rdfs:domain _:node70 .

_:node70 a owl:Class .

gr:validThrough rdfs:domain _:node73 .

_:node73 a owl:Class .

gr:appliesToPaymentMethod rdfs:domain gr:PaymentChargeSpecification .

gr:isConsumableFor rdfs:domain _:node79 .

_:node79 a owl:Class .

gr:hasValueFloat rdfs:domain gr:QuantitativeValueFloat .

gr:hasMaxValueFloat rdfs:domain gr:QuantitativeValueFloat .

gr:hasMaxValue rdfs:domain gr:QuantitativeValue .

gr:hasMinValueFloat rdfs:domain gr:QuantitativeValueFloat .

gr:hasMinValue rdfs:domain gr:QuantitativeValue .

gr:closes rdfs:domain gr:OpeningHoursSpecification .

gr:advanceBookingRequirement rdfs:domain _:node82 .

_:node82 a owl:Class .

gr:eligibleTransactionVolume rdfs:domain _:node85 .

_:node85 a owl:Class .

gr:durationOfWarrantyInMonths rdfs:domain gr:WarrantyPromise .

gr:hasGlobalLocationNumber rdfs:domain _:node89 .

_:node89 a owl:Class .

gr:isVariantOf rdfs:domain gr:ProductOrServiceModel .

gr:hasGTIN-8 rdfs:domain _:node94 .

_:node94 a owl:Class .

gr:depth rdfs:domain _:node101 .

_:node101 a owl:Class .

gr:quantitativeProductOrServiceProperty rdfs:domain _:node104 .

_:node104 a owl:Class .

gr:hasValueInteger rdfs:domain gr:QuantitativeValueInteger .

gr:hasMinValueInteger rdfs:domain gr:QuantitativeValueInteger .

gr:hasMaxValueInteger rdfs:domain gr:QuantitativeValueInteger .

gr:hasManufacturer rdfs:domain _:node107 .

_:node107 a owl:Class .

gr:description rdfs:domain _:node110 .

_:node110 a owl:Class .

gr:billingIncrement rdfs:domain gr:UnitPriceSpecification .

gr:isListPrice rdfs:domain gr:UnitPriceSpecification .

gr:color rdfs:domain _:node139 .

_:node139 a owl:Class .

gr:datatypeProductOrServiceProperty rdfs:domain _:node142 .

_:node142 a owl:Class .

gr:isAccessoryOrSparePartFor rdfs:domain _:node145 .

_:node145 a owl:Class .

gr:hasDUNS rdfs:domain _:node148 .

_:node148 a owl:Class .

gr:typeOfGood rdfs:domain gr:TypeAndQuantityNode .

gr:deliveryLeadTime rdfs:domain _:node154 .

_:node154 a owl:Class .

gr:hasStockKeepingUnit rdfs:domain _:node157 .

_:node157 a owl:Class .

gr:qualitativeProductOrServiceProperty rdfs:domain _:node162 .

_:node162 a owl:Class .

gr:availableDeliveryMethods rdfs:domain _:node166 .

_:node166 a owl:Class .

gr:includes rdfs:domain gr:Offering .

gr:hasValue rdfs:domain gr:QuantitativeValue .

gr:hasBrand rdfs:domain _:node169 .

_:node169 a owl:Class .

gr:hasOpeningHoursDayOfWeek rdfs:domain gr:OpeningHoursSpecification .

gr:priceType rdfs:domain gr:UnitPriceSpecification .

gr:eligibleRegions rdfs:domain _:node174 .

_:node174 a owl:Class .

gr:valueReference rdfs:domain _:node182 .

_:node182 a owl:Class .

gr:validFrom rdfs:domain _:node185 .

_:node185 a owl:Class .

gr:name rdfs:domain _:node191 .

_:node191 a owl:Class .

gr:hasWarrantyPromise rdfs:domain _:node220 .

_:node220 a owl:Class .

gr:hasGTIN-14 rdfs:domain _:node223 .

_:node223 a owl:Class .

gr:hasCurrencyValue rdfs:domain gr:PriceSpecification .

gr:hasMinCurrencyValue rdfs:domain gr:PriceSpecification .

gr:hasMaxCurrencyValue rdfs:domain gr:PriceSpecification .

gr:hasCurrency rdfs:domain gr:PriceSpecification .

gr:hasMakeAndModel rdfs:domain _:node227 .

_:node227 a owl:Class .

gr:valueAddedTaxIncluded rdfs:domain gr:PriceSpecification .

gr:acceptedPaymentMethods rdfs:domain _:node231 .

_:node231 a owl:Class .

gr:hasBusinessFunction rdfs:domain _:node234 .

_:node234 a owl:Class .

gr:hasWarrantyScope rdfs:domain gr:WarrantyPromise .

gr:weight rdfs:domain _:node238 .

_:node238 a owl:Class .

gr:includesObject rdfs:domain _:node241 .

_:node241 a owl:Class .

gr:hasEAN_UCC-13 rdfs:domain _:node244 .

_:node244 a owl:Class .

gr:equal rdfs:domain gr:QualitativeValue .

gr:height rdfs:domain _:node248 .

_:node248 a owl:Class .

gr:width rdfs:domain _:node251 .

_:node251 a owl:Class .

gr:hasEligibleQuantity rdfs:domain _:node254 .

_:node254 a owl:Class .

gr:eligibleDuration rdfs:domain _:node258 .

_:node258 a owl:Class .

gr:nonEqual rdfs:domain gr:QualitativeValue .

gr:condition rdfs:domain _:node262 .

_:node262 a owl:Class .

gr:appliesToDeliveryMethod rdfs:domain gr:DeliveryChargeSpecification .

gr:owns rdfs:domain _:node266 .

_:node266 a owl:Class .

gr:hasUnitOfMeasurement rdfs:domain _:node270 .

_:node270 a owl:Class .

gr:offers rdfs:domain _:node274 .

_:node274 a owl:Class .

gr:addOn rdfs:domain _:node277 .

_:node277 a owl:Class .

gr:hasNext rdfs:domain gr:DayOfWeek .

gr:hasPrevious rdfs:domain gr:DayOfWeek .

gr:lesser rdfs:domain gr:QualitativeValue .

gr:greater rdfs:domain gr:QualitativeValue .

gr:predecessorOf rdfs:domain gr:ProductOrServiceModel .

gr:successorOf rdfs:domain gr:ProductOrServiceModel .

gr:greaterOrEqual rdfs:domain gr:QualitativeValue .

gr:lesserOrEqual rdfs:domain gr:QualitativeValue .

pc:awardDate rdfs:range xsd:date .

pc:contact rdfs:range schema:ContactPoint .

pc:kind rdfs:range skos:Concept, _:node1 .

_:node1 a owl:Restriction .

pc:procedureType rdfs:range skos:Concept, _:node2 .

_:node2 a owl:Restriction .

pc:contractingAuthority rdfs:range gr:BusinessEntity .

pc:item rdfs:range gr:Offering .

pc:mainObject rdfs:range skos:Concept .

pc:additionalObject rdfs:range skos:Concept .

pc:location rdfs:range schema:Place .

pc:contractPrice rdfs:range gr:PriceSpecification .

pc:documentationPrice rdfs:range gr:PriceSpecification .

pc:tenderDeadline rdfs:range xsd:dateTime .

pc:documentationRequestDeadline rdfs:range xsd:dateTime .

pc:duration rdfs:range xsd:duration .

pc:tenderMaintenanceDuration rdfs:range xsd:duration .

pc:startDate rdfs:range xsd:date .

pc:estimatedEndDate rdfs:range xsd:date .

pc:actualEndDate rdfs:range xsd:date .

pc:awardCriteriaCombination rdfs:range pc:AwardCriteriaCombination .

pc:lot rdfs:range pc:Contract .

pc:frameworkAgreement rdfs:range pc:FrameworkAgreement .

pc:numberOfTenders rdfs:range xsd:nonNegativeInteger .

pc:tender rdfs:range pc:Tender .

pc:subsidy rdfs:range payment:Payment .

pc:agreedPrice rdfs:range gr:PriceSpecification .

pc:actualPrice rdfs:range gr:PriceSpecification .

pc:attachment rdfs:range foaf:Document .

pc:awardCriterion rdfs:range pc:CriterionWeighting .

pc:expectedNumberOfOperators rdfs:range gr:QuantitativeValueInteger .

pc:profile rdfs:range xsd:anyURI .

pc:authorityKind rdfs:range skos:Concept, _:node6 .

_:node6 a owl:Restriction .

pc:mainActivity rdfs:range skos:Concept, _:node7 .

_:node7 a owl:Restriction .

pc:offeredPrice rdfs:range gr:PriceSpecification .

gr:hasPriceSpecification rdfs:range gr:PriceSpecification .

pc:bidder rdfs:range gr:BusinessEntity .

pc:contract rdfs:range pc:Contract .

pc:weightedCriterion rdfs:range skos:Concept .

pc:criterionWeight rdfs:range pcdt:percentage .

gr:availabilityStarts rdfs:range xsd:dateTime .

gr:availableAtOrFrom rdfs:range gr:Location .

gr:taxID rdfs:range xsd:string .

gr:seeks rdfs:range gr:Offering .

gr:amountOfThisGood rdfs:range xsd:float .

gr:serialNumber rdfs:range xsd:string .

gr:hasISICv4 rdfs:range xsd:int .

gr:opens rdfs:range xsd:time .

gr:hasNAICS rdfs:range xsd:int .

gr:legalName rdfs:range rdfs:Literal .

gr:hasMPN rdfs:range xsd:string .

gr:vatID rdfs:range xsd:string .

gr:category rdfs:range rdfs:Literal .

gr:hasPOS rdfs:range gr:Location .

gr:availabilityEnds rdfs:range xsd:dateTime .

gr:eligibleCustomerTypes rdfs:range gr:BusinessEntityType .

gr:hasInventoryLevel rdfs:range gr:QuantitativeValueFloat .

gr:isSimilarTo rdfs:range gr:ProductOrService .

gr:hasOpeningHoursSpecification rdfs:range gr:OpeningHoursSpecification .

gr:validThrough rdfs:range xsd:dateTime .

gr:appliesToPaymentMethod rdfs:range gr:PaymentMethod .

gr:isConsumableFor rdfs:range gr:ProductOrService .

gr:hasValueFloat rdfs:range xsd:float .

gr:hasMaxValueFloat rdfs:range xsd:float .

gr:hasMaxValue rdfs:range rdfs:Literal .

gr:hasMinValueFloat rdfs:range xsd:float .

gr:hasMinValue rdfs:range rdfs:Literal .

gr:closes rdfs:range xsd:time .

gr:advanceBookingRequirement rdfs:range gr:QuantitativeValueInteger .

gr:eligibleTransactionVolume rdfs:range gr:PriceSpecification .

gr:durationOfWarrantyInMonths rdfs:range xsd:int .

gr:hasGlobalLocationNumber rdfs:range xsd:string .

gr:isVariantOf rdfs:range gr:ProductOrServiceModel .

gr:hasGTIN-8 rdfs:range xsd:string .

gr:depth rdfs:range gr:QuantitativeValue .

gr:quantitativeProductOrServiceProperty rdfs:range gr:QuantitativeValue .

gr:hasValueInteger rdfs:range xsd:int .

gr:hasMinValueInteger rdfs:range xsd:int .

gr:hasMaxValueInteger rdfs:range xsd:int .

gr:hasManufacturer rdfs:range gr:BusinessEntity .

gr:description rdfs:range rdfs:Literal .

gr:billingIncrement rdfs:range xsd:float .

gr:isListPrice rdfs:range xsd:boolean .

gr:color rdfs:range rdfs:Literal .

gr:datatypeProductOrServiceProperty rdfs:range rdfs:Literal .

gr:isAccessoryOrSparePartFor rdfs:range gr:ProductOrService .

gr:hasDUNS rdfs:range xsd:string .

gr:typeOfGood rdfs:range _:node151 .

_:node151 a owl:Class .

gr:deliveryLeadTime rdfs:range gr:QuantitativeValueInteger .

gr:hasStockKeepingUnit rdfs:range xsd:string .

gr:qualitativeProductOrServiceProperty rdfs:range gr:QualitativeValue .

gr:availableDeliveryMethods rdfs:range gr:DeliveryMethod .

gr:includes rdfs:range gr:ProductOrService .

gr:hasValue rdfs:range rdfs:Literal .

gr:hasBrand rdfs:range gr:Brand .

gr:hasOpeningHoursDayOfWeek rdfs:range gr:DayOfWeek .

gr:priceType rdfs:range xsd:string .

gr:eligibleRegions rdfs:range xsd:string .

gr:valueReference rdfs:range _:node179 .

_:node179 a owl:Class .

gr:validFrom rdfs:range xsd:dateTime .

gr:name rdfs:range rdfs:Literal .

gr:hasWarrantyPromise rdfs:range gr:WarrantyPromise .

gr:hasGTIN-14 rdfs:range xsd:string .

gr:hasCurrencyValue rdfs:range xsd:float .

gr:hasMinCurrencyValue rdfs:range xsd:float .

gr:hasMaxCurrencyValue rdfs:range xsd:float .

gr:hasCurrency rdfs:range xsd:string .

gr:hasMakeAndModel rdfs:range gr:ProductOrServiceModel .

gr:valueAddedTaxIncluded rdfs:range xsd:boolean .

gr:acceptedPaymentMethods rdfs:range gr:PaymentMethod .

gr:hasBusinessFunction rdfs:range gr:BusinessFunction .

gr:hasWarrantyScope rdfs:range gr:WarrantyScope .

gr:weight rdfs:range gr:QuantitativeValue .

gr:includesObject rdfs:range gr:TypeAndQuantityNode .

gr:hasEAN_UCC-13 rdfs:range xsd:string .

gr:equal rdfs:range gr:QualitativeValue;
  owl:inverseOf gr:equal .

gr:height rdfs:range gr:QuantitativeValue .

gr:width rdfs:range gr:QuantitativeValue .

gr:hasEligibleQuantity rdfs:range gr:QuantitativeValue .

gr:eligibleDuration rdfs:range gr:QuantitativeValue .

gr:nonEqual rdfs:range gr:QualitativeValue;
  owl:inverseOf gr:nonEqual .

gr:condition rdfs:range rdfs:Literal .

gr:appliesToDeliveryMethod rdfs:range gr:DeliveryMethod .

gr:owns rdfs:range gr:Individual .

gr:hasUnitOfMeasurement rdfs:range xsd:string .

gr:offers rdfs:range gr:Offering .

gr:addOn rdfs:range gr:Offering .

gr:hasNext rdfs:range gr:DayOfWeek;
  owl:inverseOf gr:hasPrevious .

gr:hasPrevious rdfs:range gr:DayOfWeek;
  owl:inverseOf gr:hasNext .

gr:lesser rdfs:range gr:QualitativeValue;
  owl:inverseOf gr:greater .

gr:greater rdfs:range gr:QualitativeValue;
  owl:inverseOf gr:lesser .

gr:predecessorOf rdfs:range gr:ProductOrServiceModel;
  owl:inverseOf gr:successorOf .

gr:successorOf rdfs:range gr:ProductOrServiceModel;
  owl:inverseOf gr:predecessorOf .

gr:greaterOrEqual rdfs:range gr:QualitativeValue;
  owl:inverseOf gr:lesserOrEqual .

gr:lesserOrEqual rdfs:range gr:QualitativeValue;
  owl:inverseOf gr:greaterOrEqual .

pc:tenderDeadline owl:equivalentProperty loted:DT .

pc:awardCriterion owl:equivalentProperty loted:AC .

schema:manufacturer owl:equivalentProperty gr:hasManufacturer .

schema:description owl:equivalentProperty gr:description .

schema:name owl:equivalentProperty gr:name .

schema:image owl:equivalentProperty foaf:depiction .

pc:Contract owl:equivalentClass loted:Tender .

pc:AwardCriteriaCombination owl:equivalentClass loted:AwardCriteria .

gr:BusinessEntity owl:equivalentClass _:node280 .

_:node280 a owl:Class .

schema:Place owl:equivalentClass gr:Location .

gr:Location owl:equivalentClass gr:LocationOfSalesOrServiceProvisioning .

gr:Individual owl:equivalentClass gr:ActualProductOrServiceInstance .

schema:Product owl:equivalentClass gr:ProductOrService .

gr:SomeItems owl:equivalentClass gr:ProductOrServicesSomeInstancesPlaceholder .

gr:LocationOfSalesOrServiceProvisioning owl:equivalentClass gr:Location .

gr:ProductOrServicesSomeInstancesPlaceholder owl:equivalentClass gr:SomeItems .

gr:ActualProductOrServiceInstance owl:equivalentClass gr:Individual .

_:node165 a gr:Offering .

_:node4 rdf:first pc:Contract .

_:node5 rdf:first pc:Tender .

_:node9 rdf:first gr:Offering .

_:node10 rdf:first schema:Offer .

_:node12 rdf:first gr:Offering .

_:node13 rdf:first schema:Offer .

_:node15 rdf:first gr:BusinessEntity .

_:node16 rdf:first schema:Organization .

_:node17 rdf:first schema:Person .

_:node19 rdf:first gr:BusinessEntity .

_:node20 rdf:first schema:Organization .

_:node21 rdf:first schema:Person .

_:node23 rdf:first gr:Individual .

_:node24 rdf:first gr:Offering .

_:node25 rdf:first schema:Product .

_:node27 rdf:first gr:BusinessEntity .

_:node28 rdf:first gr:Location .

_:node29 rdf:first schema:Organization .

_:node30 rdf:first schema:Place .

_:node32 rdf:first gr:BusinessEntity .

_:node33 rdf:first schema:Organization .

_:node35 rdf:first gr:BusinessEntity .

_:node36 rdf:first schema:Organization .

_:node38 rdf:first gr:Offering .

_:node39 rdf:first gr:ProductOrService .

_:node40 rdf:first schema:Product .

_:node42 rdf:first gr:BusinessEntity .

_:node43 rdf:first schema:Organization .

_:node44 rdf:first schema:Person .

_:node46 rdf:first gr:ProductOrService .

_:node47 rdf:first gr:Offering .

_:node48 rdf:first gr:Location .

_:node49 rdf:first gr:BusinessEntity .

_:node50 rdf:first schema:Offer .

_:node51 rdf:first schema:Product .

_:node52 rdf:first schema:Place .

_:node53 rdf:first schema:Organization .

_:node55 rdf:first gr:BusinessEntity .

_:node56 rdf:first schema:Organization .

_:node58 rdf:first gr:Offering .

_:node59 rdf:first schema:Offer .

_:node61 rdf:first gr:Offering .

_:node62 rdf:first schema:Offer .

_:node64 rdf:first gr:Offering .

_:node65 rdf:first gr:SomeItems .

_:node66 rdf:first schema:Offer .

_:node68 rdf:first gr:ProductOrService .

_:node69 rdf:first schema:Product .

_:node71 rdf:first gr:Location .

_:node72 rdf:first schema:Place .

_:node74 rdf:first gr:Offering .

_:node75 rdf:first gr:OpeningHoursSpecification .

_:node76 rdf:first gr:PriceSpecification .

_:node77 rdf:first gr:License .

_:node78 rdf:first schema:Offer .

_:node80 rdf:first gr:ProductOrService .

_:node81 rdf:first schema:Product .

_:node83 rdf:first gr:Offering .

_:node84 rdf:first schema:Offer .

_:node86 rdf:first gr:Offering .

_:node87 rdf:first gr:PriceSpecification .

_:node88 rdf:first schema:Offer .

_:node90 rdf:first gr:BusinessEntity .

_:node91 rdf:first gr:Location .

_:node92 rdf:first schema:Place .

_:node93 rdf:first schema:Organization .

_:node95 rdf:first gr:Offering .

_:node96 rdf:first gr:ProductOrService .

_:node97 rdf:first schema:Product .

_:node99 rdf:first gr:Offering .

_:node100 rdf:first schema:Offer .

_:node102 rdf:first gr:ProductOrService .

_:node103 rdf:first schema:Product .

_:node105 rdf:first gr:ProductOrService .

_:node106 rdf:first schema:Product .

_:node108 rdf:first gr:ProductOrService .

_:node109 rdf:first schema:Product .

_:node111 rdf:first owl:Thing .

_:node112 rdf:first gr:Brand .

_:node113 rdf:first gr:BusinessEntity .

_:node114 rdf:first gr:BusinessEntityType .

_:node115 rdf:first gr:BusinessFunction .

_:node116 rdf:first gr:DayOfWeek .

_:node117 rdf:first gr:DeliveryChargeSpecification .

_:node118 rdf:first gr:DeliveryMethod .

_:node119 rdf:first gr:DeliveryModeParcelService .

_:node120 rdf:first gr:Individual .

_:node121 rdf:first gr:Location .

_:node122 rdf:first gr:Offering .

_:node123 rdf:first gr:OpeningHoursSpecification .

_:node124 rdf:first gr:PaymentChargeSpecification .

_:node125 rdf:first gr:PaymentMethod .

_:node126 rdf:first gr:PaymentMethodCreditCard .

_:node127 rdf:first gr:PriceSpecification .

_:node128 rdf:first gr:ProductOrService .

_:node129 rdf:first gr:ProductOrServiceModel .

_:node130 rdf:first gr:QualitativeValue .

_:node131 rdf:first gr:QuantitativeValue .

_:node132 rdf:first gr:QuantitativeValueFloat .

_:node133 rdf:first gr:QuantitativeValueInteger .

_:node134 rdf:first gr:SomeItems .

_:node135 rdf:first gr:TypeAndQuantityNode .

_:node136 rdf:first gr:UnitPriceSpecification .

_:node137 rdf:first gr:WarrantyPromise .

_:node138 rdf:first gr:WarrantyScope .

_:node140 rdf:first gr:ProductOrService .

_:node141 rdf:first schema:Product .

_:node143 rdf:first gr:ProductOrService .

_:node144 rdf:first schema:Product .

_:node146 rdf:first gr:ProductOrService .

_:node147 rdf:first schema:Product .

_:node149 rdf:first gr:BusinessEntity .

_:node150 rdf:first schema:Organization .

_:node152 rdf:first gr:Individual .

_:node153 rdf:first gr:SomeItems .

_:node155 rdf:first gr:Offering .

_:node156 rdf:first schema:Offer .

_:node158 rdf:first gr:Offering .

_:node159 rdf:first gr:ProductOrService .

_:node160 rdf:first schema:Offer .

_:node161 rdf:first schema:Product .

_:node163 rdf:first gr:ProductOrService .

_:node164 rdf:first schema:Product .

_:node167 rdf:first gr:Offering .

_:node168 rdf:first schema:Offer .

_:node170 rdf:first gr:BusinessEntity .

_:node171 rdf:first gr:ProductOrService .

_:node172 rdf:first schema:Organization .

_:node173 rdf:first schema:Product .

_:node175 rdf:first gr:DeliveryChargeSpecification .

_:node176 rdf:first gr:Offering .

_:node177 rdf:first gr:License .

_:node178 rdf:first schema:Offer .

_:node180 rdf:first gr:QualitativeValue .

_:node181 rdf:first gr:QuantitativeValue .

_:node183 rdf:first gr:QualitativeValue .

_:node184 rdf:first gr:QuantitativeValue .

_:node186 rdf:first gr:Offering .

_:node187 rdf:first gr:OpeningHoursSpecification .

_:node188 rdf:first gr:PriceSpecification .

_:node189 rdf:first gr:License .

_:node190 rdf:first schema:Offer .

_:node192 rdf:first owl:Thing .

_:node193 rdf:first gr:Brand .

_:node194 rdf:first gr:BusinessEntity .

_:node195 rdf:first gr:BusinessEntityType .

_:node196 rdf:first gr:BusinessFunction .

_:node197 rdf:first gr:DayOfWeek .

_:node198 rdf:first gr:DeliveryChargeSpecification .

_:node199 rdf:first gr:DeliveryMethod .

_:node200 rdf:first gr:DeliveryModeParcelService .

_:node201 rdf:first gr:Individual .

_:node202 rdf:first gr:Location .

_:node203 rdf:first gr:Offering .

_:node204 rdf:first gr:OpeningHoursSpecification .

_:node205 rdf:first gr:PaymentChargeSpecification .

_:node206 rdf:first gr:PaymentMethod .

_:node207 rdf:first gr:PaymentMethodCreditCard .

_:node208 rdf:first gr:PriceSpecification .

_:node209 rdf:first gr:ProductOrService .

_:node210 rdf:first gr:ProductOrServiceModel .

_:node211 rdf:first gr:QualitativeValue .

_:node212 rdf:first gr:QuantitativeValue .

_:node213 rdf:first gr:QuantitativeValueFloat .

_:node214 rdf:first gr:QuantitativeValueInteger .

_:node215 rdf:first gr:SomeItems .

_:node216 rdf:first gr:TypeAndQuantityNode .

_:node217 rdf:first gr:UnitPriceSpecification .

_:node218 rdf:first gr:WarrantyPromise .

_:node219 rdf:first gr:WarrantyScope .

_:node221 rdf:first gr:Offering .

_:node222 rdf:first schema:Offer .

_:node224 rdf:first gr:Offering .

_:node225 rdf:first gr:ProductOrService .

_:node226 rdf:first schema:Product .

_:node228 rdf:first gr:Individual .

_:node229 rdf:first gr:SomeItems .

_:node230 rdf:first schema:Product .

_:node232 rdf:first gr:Offering .

_:node233 rdf:first schema:Offer .

_:node235 rdf:first gr:Offering .

_:node236 rdf:first gr:TypeAndQuantityNode .

_:node237 rdf:first schema:Offer .

_:node239 rdf:first gr:ProductOrService .

_:node240 rdf:first schema:Product .

_:node242 rdf:first gr:Offering .

_:node243 rdf:first schema:Offer .

_:node245 rdf:first gr:Offering .

_:node246 rdf:first gr:ProductOrService .

_:node247 rdf:first schema:Product .

_:node249 rdf:first gr:ProductOrService .

_:node250 rdf:first schema:Product .

_:node252 rdf:first gr:ProductOrService .

_:node253 rdf:first schema:Product .

_:node255 rdf:first gr:Offering .

_:node256 rdf:first gr:PriceSpecification .

_:node257 rdf:first schema:Offer .

_:node259 rdf:first gr:Offering .

_:node260 rdf:first gr:License .

_:node261 rdf:first schema:Offer .

_:node263 rdf:first gr:Offering .

_:node264 rdf:first gr:ProductOrService .

_:node265 rdf:first schema:Product .

_:node267 rdf:first gr:BusinessEntity .

_:node268 rdf:first schema:Organization .

_:node269 rdf:first schema:Person .

_:node271 rdf:first gr:QuantitativeValue .

_:node272 rdf:first gr:TypeAndQuantityNode .

_:node273 rdf:first gr:UnitPriceSpecification .

_:node275 rdf:first gr:BusinessEntity .

_:node276 rdf:first schema:Organization .

_:node278 rdf:first gr:Offering .

_:node279 rdf:first schema:Offer .

_:node281 rdf:first schema:Person .

_:node282 rdf:first schema:Organization .

_:node4 rdf:rest _:node5 .

_:node5 rdf:rest rdf:nil .

_:node9 rdf:rest _:node10 .

_:node10 rdf:rest rdf:nil .

_:node12 rdf:rest _:node13 .

_:node13 rdf:rest rdf:nil .

_:node15 rdf:rest _:node16 .

_:node16 rdf:rest _:node17 .

_:node17 rdf:rest rdf:nil .

_:node19 rdf:rest _:node20 .

_:node20 rdf:rest _:node21 .

_:node21 rdf:rest rdf:nil .

_:node23 rdf:rest _:node24 .

_:node24 rdf:rest _:node25 .

_:node25 rdf:rest rdf:nil .

_:node27 rdf:rest _:node28 .

_:node28 rdf:rest _:node29 .

_:node29 rdf:rest _:node30 .

_:node30 rdf:rest rdf:nil .

_:node32 rdf:rest _:node33 .

_:node33 rdf:rest rdf:nil .

_:node35 rdf:rest _:node36 .

_:node36 rdf:rest rdf:nil .

_:node38 rdf:rest _:node39 .

_:node39 rdf:rest _:node40 .

_:node40 rdf:rest rdf:nil .

_:node42 rdf:rest _:node43 .

_:node43 rdf:rest _:node44 .

_:node44 rdf:rest rdf:nil .

_:node46 rdf:rest _:node47 .

_:node47 rdf:rest _:node48 .

_:node48 rdf:rest _:node49 .

_:node49 rdf:rest _:node50 .

_:node50 rdf:rest _:node51 .

_:node51 rdf:rest _:node52 .

_:node52 rdf:rest _:node53 .

_:node53 rdf:rest rdf:nil .

_:node55 rdf:rest _:node56 .

_:node56 rdf:rest rdf:nil .

_:node58 rdf:rest _:node59 .

_:node59 rdf:rest rdf:nil .

_:node61 rdf:rest _:node62 .

_:node62 rdf:rest rdf:nil .

_:node64 rdf:rest _:node65 .

_:node65 rdf:rest _:node66 .

_:node66 rdf:rest rdf:nil .

_:node68 rdf:rest _:node69 .

_:node69 rdf:rest rdf:nil .

_:node71 rdf:rest _:node72 .

_:node72 rdf:rest rdf:nil .

_:node74 rdf:rest _:node75 .

_:node75 rdf:rest _:node76 .

_:node76 rdf:rest _:node77 .

_:node77 rdf:rest _:node78 .

_:node78 rdf:rest rdf:nil .

_:node80 rdf:rest _:node81 .

_:node81 rdf:rest rdf:nil .

_:node83 rdf:rest _:node84 .

_:node84 rdf:rest rdf:nil .

_:node86 rdf:rest _:node87 .

_:node87 rdf:rest _:node88 .

_:node88 rdf:rest rdf:nil .

_:node90 rdf:rest _:node91 .

_:node91 rdf:rest _:node92 .

_:node92 rdf:rest _:node93 .

_:node93 rdf:rest rdf:nil .

_:node95 rdf:rest _:node96 .

_:node96 rdf:rest _:node97 .

_:node97 rdf:rest rdf:nil .

_:node99 rdf:rest _:node100 .

_:node100 rdf:rest rdf:nil .

_:node102 rdf:rest _:node103 .

_:node103 rdf:rest rdf:nil .

_:node105 rdf:rest _:node106 .

_:node106 rdf:rest rdf:nil .

_:node108 rdf:rest _:node109 .

_:node109 rdf:rest rdf:nil .

_:node111 rdf:rest _:node112 .

_:node112 rdf:rest _:node113 .

_:node113 rdf:rest _:node114 .

_:node114 rdf:rest _:node115 .

_:node115 rdf:rest _:node116 .

_:node116 rdf:rest _:node117 .

_:node117 rdf:rest _:node118 .

_:node118 rdf:rest _:node119 .

_:node119 rdf:rest _:node120 .

_:node120 rdf:rest _:node121 .

_:node121 rdf:rest _:node122 .

_:node122 rdf:rest _:node123 .

_:node123 rdf:rest _:node124 .

_:node124 rdf:rest _:node125 .

_:node125 rdf:rest _:node126 .

_:node126 rdf:rest _:node127 .

_:node127 rdf:rest _:node128 .

_:node128 rdf:rest _:node129 .

_:node129 rdf:rest _:node130 .

_:node130 rdf:rest _:node131 .

_:node131 rdf:rest _:node132 .

_:node132 rdf:rest _:node133 .

_:node133 rdf:rest _:node134 .

_:node134 rdf:rest _:node135 .

_:node135 rdf:rest _:node136 .

_:node136 rdf:rest _:node137 .

_:node137 rdf:rest _:node138 .

_:node138 rdf:rest rdf:nil .

_:node140 rdf:rest _:node141 .

_:node141 rdf:rest rdf:nil .

_:node143 rdf:rest _:node144 .

_:node144 rdf:rest rdf:nil .

_:node146 rdf:rest _:node147 .

_:node147 rdf:rest rdf:nil .

_:node149 rdf:rest _:node150 .

_:node150 rdf:rest rdf:nil .

_:node152 rdf:rest _:node153 .

_:node153 rdf:rest rdf:nil .

pc:Contract rdfs:comment "Instance této třídy je abstraktní informační entitou o veřejné zakázce. Obsahuje všechny aktuálně známé informace o zakázce, tj. např. o zadavateli veřejné zakázky, službách či dodávkách, které ve veřejné zakázce nakupuje, a o podmínkách nákupu (termíny, očekávané ceny, atd.). Dále obsahuje informace o nabídkách od zájemců o zakázku a o vybrané nabídce. Pokud již byla zakázka realizována, obsahuje i informace o skutečné ceně za realizaci apod."@cs,
    "An instance of this class is an abstract information entity about a public contract. It consists of all currently known information about a contract, e.g., a contracting authority, services or supplies which shall be purchased, and contract conditions (e.g., important dates, expected price, etc.). It also informs about tenders received from particular bidders and about an accepted tender. If the contract has already been realized it also informs about an actual price of realization, etc."@en .

pc:FrameworkAgreement rdfs:comment "Třída pro popis rámcové smlouvy"@cs, "Class for decribing a framework agreement"@en .

pc:Tender rdfs:comment "Základní třída pro popis nabídky zájemce o zakázku"@cs, "Basic class for decribing a tender submitted by a bidder"@en .

gr:Offering rdfs:comment """An offering represents the public, not necessarily binding, not necessarily exclusive, announcement by a gr:BusinessEntity to provide (or seek) a certain gr:BusinessFunction for a certain gr:ProductOrService to a specified target audience. An offering is specified by the type of product or service or bundle it refers to, what business function is being offered (sales, rental, ...), and a set of commercial properties. It can either refer to 
(1) a clearly specified instance (gr:Individual),
(2) to a set of anonymous instances of a given type (gr:SomeItems),
(3) a product model specification (gr:ProductOrServiceModel), see also section 3.3.3 of the GoodRelations Technical Report. 

An offering may be constrained in terms of the eligible type of business partner, countries, quantities, and other commercial properties. The definition of the commercial properties, the type of product offered, and the business function are explained in other parts of this vocabulary in more detail.

Example: Peter Miller offers to repair TV sets made by Siemens, Volkswagen Innsbruck sells a particular instance of a Volkswagen Golf at $10,000.

Compatibility with schema.org: This class is a superclass to http://schema.org/Offer, since gr:Offering can also represent demand."""@en .

pc:AwardCriteriaCombination rdfs:comment "Třída pro popis kombinace kritérií pro posuzování nabídek zájemců o zakázku"@cs,
    "Class for description of criteria combination used for tender evaluation"@en .

pc:CriterionWeighting rdfs:comment "Třída pro popis jednoho kritéria a jeho váhy."@cs,
    "Class for description of one criterion and its weight"@en .

pc:TendersOpening rdfs:comment "Opening of tenders submitted for a public contract"@en,
    "Otevírání nabídek zaslaných pro veřejnou zakázku"@cs .

pc:awardDate rdfs:comment "Vlastnost pro datum přidělení zakázky dodavateli. Kardinalita 0..1"@cs,
    "Property for date of contract award to a bidder. Cardinality 0..1"@en .

pc:contact rdfs:comment "Vlastnost pro kontaktní údaje na místo nebo osobu určenou pro komunikaci s veřejností a zájemci o zakázku. Pokud je kontaktních míst či osob více (např. pro vyzvednutí dokumentace k veřejné zakázce), je pro každou uveden samostatný kontakt. Kardinalita 0..*"@cs,
    "Property for contact information for a person or place responsible for a communication with the public and bidders. If there are more contact places or persons (e.g., for collecting documentation to the public contract), there is a separate contact for each person. Cardinality 0..*"@en .

pc:kind rdfs:comment "Kategorie veřejné zakázky specifikuje základní zaměření veřejné zakázky na stavební práce, dodávku zboží nebo služby. Lze použít pouze jeden z předdefinovaných SKOS konceptů. Kardinalita 0..1"@cs,
    "Kind of a public contract specifies a basic focus of the contract on works, supplies or services. Only a predefined SKOS concept can be used. Cardinality 0..1"@en .

pc:procedureType rdfs:comment "Druh řízení veřejné zakázky specifikuje proceduru, podle které je zakázka uveřejňována a podle které je vybírán dodavatel. Lze použít pouze jednu z předdefinovaných hodnot. Kardinalita 0..1"@cs,
    "Type of procedure of a public contract specifies a procedure which is applied to publish information about the contract and choose a supplier. Only a predefined value can be used. Cardinality 0..1"@en .

pc:contractingAuthority rdfs:comment "Instituce, která vypisuje veřejnou zakázku, přijímá nabídky a vybírá vhodného dodavatele na základě pravidel stanovených zakázkou. Kardinalita 0..1"@cs,
    "Institution which issues a public contract, receives tenders to the contract and chooses a suitable supplier on the base of the conditions given by the contract. Cardinality 0..1"@en .

gr:BusinessEntity rdfs:comment """An instance of this class represents the legal agent making (or seeking) a particular offering. This can be a legal body or a person. A business entity has at least a primary mailing address and contact details. For this, typical address standards (vCard) and location data (geo, WGS84) can be attached. Note that the location of the business entity is not necessarily the location from which the product or service is being available (e.g. the branch or store). Use gr:Location for stores and branches.
		
Example: Siemens Austria AG, Volkswagen Ltd., Peter Miller's Cell phone Shop LLC

Compatibility with schema.org: This class is equivalent to the union of http://schema.org/Person and http://schema.org/Organization.		
"""@en .

pc:item rdfs:comment "Položka poptávaná v rámci veřejné zakázky. Může být kombinací několika produktů či služeb, což lze vyjádřit pomocí vlastností gr:Offering. Kardinalita 0..*"@cs,
    "An item inquired by a public contract. It can be a combination of several products or services which can be expressed using properties of gr:Offering. Cardinality 0..*"@en .

pc:mainObject rdfs:comment "CPV (Common Procurement Vocabulary) kód popisující hlavní předmět veřejné zakázky. Kardinalita 0..1"@cs,
    "CPV (Common Procurement Vocabulary) code describing the main object of a public contract. Cardinality 0..1"@en .

pc:additionalObject rdfs:comment "CPV (Common Procurement Vocabulary) kód popisující doplňující předmět veřejné zakázky. Kardinalita 0..*"@cs,
    "CPV (Common Procurement Vocabulary) code describing an additional object of a public contract. Cardinality 0..*"@en .

pc:location rdfs:comment "Místo, kde dojde k dodání produktu nebo plnění služby nasmlouvané ve veřejné zakázce. Kardinalita 0..*"@cs,
    "Place of delivery of contracted product or performance of contracted service. Cardinality 0..*"@en .

pc:contractPrice rdfs:comment "Abstraktní vlastnost pro cenu přiřazené k veřejné zakázce"@cs,
    "Abstract property for price of public contract"@en .

gr:PriceSpecification rdfs:comment "The superclass of all price specifications."@en .

pc:documentationPrice rdfs:comment "Vlastnost pro cenu zadávací dokumentace k zakázce. Kardinalita 0..1"@cs,
    "Property for price of documentation for public contract. Cardinality 0..1"@en .

pc:estimatedPrice rdfs:comment "Vlastnost pro odhadovanou cenu veřejné zakázky. Může jít o přesně odhadovanou částku nebo interval. Kardinalita 0..1"@cs,
    "Property for estimated price of public contract. It can be an exact estimation or an interval. Cardinality 0..1"@en .

pc:tenderDeadline rdfs:comment "Vlastnost pro lhůtu pro doručení nabídek nebo přijetí žádostí o účast. Kardinalita 0..1"@cs,
    "Property for time limit for receipt of tenders or requests to participate. Cardinality 0..1"@en .

pc:documentationRequestDeadline rdfs:comment "Vlastnost pro lhůtu pro vyžádání dokumentace k veřejné zakázce. Kardinalita 0..1"@cs,
    "Property for time limit for receipt of requests for documentation. Cardinality 0..1"@en .

pc:duration rdfs:comment "Vlastnost pro dobu trvání zakázky. Doba trvání může být uvedena ve dnech, měsících, letech apod. Kardinalita 0..1"@cs,
    "Property for duration of contract. The duration may be described in days, months, years, etc. Cardinality 0..1"@en .

pc:tenderMaintenanceDuration rdfs:comment "Vlastnost pro vyjádření minimální doby, po kterou je uchazeč svou nabídkou vázán. Doba trvání může být uvedena ve dnech, měsících, letech apod. Kardinalita 0..1"@cs,
    "Property for expressing minimum time frame during which the tenderer must maintain the tender. The duration may be described in days, months, years, etc. Cardinality 0..1"@en .

pc:startDate rdfs:comment "Vlastnost pro datum začátku realizace zakázky, které je uvedené ve smlouvě. Kardinalita 0..1"@cs,
    "Property for start date of public contract realization coming from the contract's text. Cardinality 0..1"@en .

pc:estimatedEndDate rdfs:comment "Vlastnost pro očekávané datum konce realizace zakázky. Kardinalita 0..1"@cs,
    "Property for estimated end date of public contract realization. Cardinality 0..1"@en .

pc:actualEndDate rdfs:comment "Vlastnost pro skutečné datum konce realizace zakázky. Kardinalita 0..1"@cs,
    "Property for actual end date of public contract's realization. Cardinality 0..1"@en .

pc:awardCriteriaCombination rdfs:comment "Vlastnost pro nastavení kombinace kritérií pro hodnocení nabídek zájemců o zakázku. Kardinalita 0..1"@cs,
    "Property for criteria combination for tender evaluation. Cardinality 0..1"@en .

pc:lot rdfs:comment "Vlastnost pro specifikaci části zakázky. Zakázku rozděluje na části zadavatel, pokud je zakázka přiliš velká. Zájemci o zakázku podávají nabídky na každou část odděleně a pro každou část zakázky je vybrán samostatný dodavatel. Pro samotnou zakázku nabídky nejsou podávány. Kardinalita 0..*"@cs,
    "Property for specifying contract lot. When contract is too big, it is split to lots by contracting authority. Bidders then tender each lot separately. For each lot the authority awards a separate tender. The contract itself has no tenders. Cardinality 0..*"@en .

pc:frameworkAgreement rdfs:comment "Vlastnost pro rámcovou smlouvu, na jejímž základě byla veřejná zakázka zadána. Kardinalita 0..1"@cs,
    "Property for a framework agreement on which base a public contract was issued. Cardinality 0..1"@en .

pc:numberOfTenders rdfs:comment "Vlastnost pro počet obdržených nabídek. Kardinalita 0..1"@cs,
    "Property for number of tenders received. Cardinality 0..1"@en .

pc:tender rdfs:comment "Vlastnost pro nabídku zájemce o zakázku. Kardinalita 0..*"@cs,
    "Property for a tender submitted by a bidder. Cardinality 0..*"@en .

pc:awardedTender rdfs:comment "Vlastnost pro vítěznou nabídku zájemce o zakázku. Kardinalita 0..1"@cs,
    "Property for awarded tender submitted by a bidder. Cardinality 0..1"@en .

pc:subsidy rdfs:comment "Vlastnost pro dotaci použitou pro zakázku. Kardinalita 0..*"@cs,
    "Property for used tender subsidy. Cardinality 0..*"@en .

pc:agreedPrice rdfs:comment "Vlastnost pro cenu napsanou na smlouvě s dodavatelem. Kardinalita 0..1"@cs,
    "Property for a price stated on the contract with the supplier. Cardinality 0..1"@en .

pc:actualPrice rdfs:comment "Vlastnost pro skutečnou cenu zaplacenou za zakázku. Kardinalita 0..1"@cs,
    "Property for actual price of the public contract. Cardinality 0..1"@en .

pc:attachment rdfs:comment "Vlastnost pro připojení ostatních příloh. Zadávací dokumentaci připojte pomocí pc:specification, smlouvu pomocí pc:agreement. Kardinalita 0..*"@cs,
    "Property for attachment of other documents. For attachment of contract specification use pc:specification. For attachment of contract agreement use pc:agreement. Cardinality 0..*"@en .

pc:specification rdfs:comment "Vlastnost pro připojení dokumentů obsahujících zadávací dokumentaci veřejné zakázky. Kardinalita 0..*"@cs,
    "Property for attachment of documents containing the contract specification. Cardinality 0..*"@en .

pc:agreement rdfs:comment "Vlastnost pro připojení dokumentů obsahujících smlouvy na veřejnou zakázku uzavřené mezi zadavatelem a dodavatelem. Kardinalita 0..*"@cs,
    "Property for attachment of documents containing the agreement between supplier and contractor. Cardinality 0..*"@en .

pc:awardCriterion rdfs:comment "Vlastnost pro nastavení jednoho kritéria pro hodnocení nabídek zájemců o zakázku. Kardinalita 0..*"@cs,
    "Property for setting a criterion for tender evaluation. Cardinality 0..*"@en .

pc:expectedNumberOfOperators rdfs:comment "Očekávaný počet účastníků rámcové smlouvy. Kardinalita 0..1"@cs,
    "Expected number of operators of framework agreement. Cardinality 0..1"@en .

gr:QuantitativeValueInteger rdfs:comment """An instance of this class is an actual integer value for a quantitative property of a product. This instance is usually characterized by a minimal value, a maximal value, and a unit of measurement. 

Example: A seating capacity between 1 and 8 persons.

Note: Users must keep in mind that ranges in here mean that ALL possible values in this interval are covered. (Sometimes, the actual commitment may be less than that: \"We sell cars from 2 - 12 seats\" does often not really mean that they have cars with 2,3,4,...12 seats.). Someone renting out two types of rowing boats, one that fits for 1 or 2 people, and another that must be operated by 4 people cannot claim to rent boats with a seating capacity between 1 and 4 people. He or she is offering two boat types for 1-2 and 4 persons.
		
Compatibility with schema.org: This class is a subclass of http://schema.org/Quantity."""@en .

pc:profile rdfs:comment "Vlastnost pro internetovou adresu profilové stránky zadavatele veřejných zakázek (URL)."@cs,
    "Property for the internet address of the profile of contracting authority (URL)."@en .

pc:authorityKind rdfs:comment "Vlastnost pro druh zadavatele. Lze použít pouze jeden z předdefinovaných SKOS konceptů. Kardinalita 0..1"@cs,
    "Property for a kind of a contracting authority. Only a predefined SKOS concept can be used. Cardinality 0..1"@en .

pc:mainActivity rdfs:comment "Vlastnost pro hlavní aktivitu zadavatele. Lze použít pouze jeden z předdefinovaných SKOS konceptů. Kardinalita 0..1"@cs,
    "Property for main activity of contracting authority. Only a predefined SKOS concept can be used. Cardinality 0..1"@en .

pc:offeredPrice rdfs:comment "Vlastnost pro cenu nabídnutou zájemcem o zakázku. Kardinalita 0..1"@cs,
    "Property for price offered by supplier. Cardinality 0..1"@en .

gr:hasPriceSpecification rdfs:comment """This links a gr:Offering to a gr:PriceSpecification or specifications. There can be unit price specifications, payment charge specifications, and delivery charge specifications. For each type, multiple specifications for the same gr:Offering are possible, e.g. for different quantity ranges or for different currencies, or for different combinations of gr:DeliveryMethod and target destinations.

Recommended retail prices etc. can be marked by the gr:priceType property of the gr:UnitPriceSpecification."""@en .

pc:bidder rdfs:comment "Vlastnost pro zájemce o zakázku podávajícího nabídku. Kardinalita 0..1"@cs,
    "Property for bidder submitting the tender. Cardinality 0..1"@en .

pc:contract rdfs:comment "Public contract, for which tenders are opened"@en, "Veřejná zakázka, pro níž jsou otevírány nabídky"@cs .

pc:weightedCriterion rdfs:comment "Vlastnost pro připojení kritéria, které je váženo. Kardinalita 0..1"@cs,
    "Property for attaching criterion that is weighted. Cardinality 0..1"@en .

pc:criterionWeight rdfs:comment "Vlastnost pro specifikaci váhy kritéria pro hodnocení nabídky. Kardinalita 0..1"@cs,
    "Property for criterion weight for tender evaluation. Cardinality 0..1"@en .

gr:availabilityStarts rdfs:comment """This property specifies the beginning of the availability of the gr:ProductOrService included in the gr:Offering.
The difference to the properties gr:validFrom and gr:validThrough is that those specify the period of time during which the offer is valid and can be accepted.

Example: I offer to lease my boat for the period of August 1 - August 31, 2010, but you must accept by offer no later than July 15.

A time-zone should be specified. For a time in GMT/UTC, simply add a \"Z\" following the time:

2008-05-30T09:30:10Z.

Alternatively, you can specify an offset from the UTC time by adding a positive or negative time following the time:

2008-05-30T09:30:10-09:00

or

2008-05-30T09:30:10+09:00.

Note: There is another property gr:availableAtOrFrom, which is used to indicate the gr:Location (e.g. store or shop) from which the goods would be available."""@en .

<http://purl.org/goodrelations/v1> rdfs:comment """The GoodRelations ontology provides the vocabulary for annotating e-commerce offerings (1) to sell, lease, repair, dispose, or maintain commodity products and (2) to provide commodity services.

GoodRelations allows describing the relationship between (1) Web resources, (2) offerings made by those Web resources, (3) legal entities, (4) prices, (5) terms and conditions, and the aforementioned ontologies for products and services (6).
 
For more information, see http://purl.org/goodrelations/

Note: The base URI of GoodRelations is http://purl.org/goodrelations/v1. Please make sure you are only using element identifiers in this namespace, e.g. http://purl.org/goodrelations/v1#BusinessEntity. There may be copies of the ontology file on the Web which can be retrieved from other locations, BUT THOSE LOCATIONS MUST NOT BE USED AS THE BASIS OF IDENTIFIERS.

If you use GoodRelations for scientific purposes, please cite our paper:

Hepp, Martin: GoodRelations: An Ontology for Describing Products and Services Offers on the Web, Proceedings of the 16th International Conference on Knowledge Engineering and Knowledge Management (EKAW2008), September 29 - October 3, 2008, Acitrezza, Italy, Springer LNCS, Vol. 5268, pp. 332-347.

PDF at http://www.heppnetz.de/publications/"""@en .

gr:availableAtOrFrom rdfs:comment "This states that a particular gr:Offering is available at or from the given gr:Location (e.g. shop or branch)."@en .

gr:Location rdfs:comment """A location is a point or area of interest from which a particular product or service is available, e.g. a store, a bus stop, a gas station, or a ticket booth. The difference to gr:BusinessEntity is that the gr:BusinessEntity is the legal entity (e.g. a person or corporation) making the offer, while gr:Location is the store, office, or place. A chain restaurant will e.g. have one legal entity but multiple restaurant locations. Locations are characterized by an address or geographical position and a set of opening hour specifications for various days of the week.
		
Example: A rental car company may offer the Business Function Lease Out of cars from two locations, one in Fort Myers, Florida, and one in Boston, Massachussetts. Both stations are open 7:00 - 23:00 Mondays through Saturdays.

Note: Typical address standards (vcard) and location data (geo, WGC84) should be attached to a gr:Location node. Since there already exist established vocabularies for this, the GoodRelations ontology does not provide respective attributes. Instead, the use of respective vocabularies is recommended. However, the gr:hasGlobalLocationNumber property is  provided for linking to public identifiers for business locations.
		
Compatibility with schema.org: This class is equivalent to http://schema.org/Place."""@en .

gr:taxID rdfs:comment "The Tax / Fiscal ID of the gr:BusinessEntity, e.g. the TIN in the US or the CIF/NIF in Spain. It is usually assigned by the country of residence"@en .

gr:seeks rdfs:comment "This links a gr:BusinessEntity to gr:Offering nodes that describe what the business entity is interested in (i.e., the buy side). If you want to express interest in offering something, use gr:offers instead. Note that this substitutes the former gr:BusinessFunction gr:Buy, which is now deprecated."@en .

gr:Reseller rdfs:comment "The gr:BusinessEntityType representing such agents that are purchasing the scope of products included in the gr:Offering for resale on the market. Resellers are also businesses, i.e., they are officially registered with the public administration and strive for profits by their activities."@en .

gr:BusinessEntityType rdfs:comment """A business entity type is a conceptual entity representing the legal form, the size, the main line of business, the position in the value chain, or any combination thereof, of a gr:BusinessEntity. From the ontological point of view, business entity types are mostly roles that a business entity has in the market. Business entity types are important for specifying eligible customers, since a gr:Offering is often valid only for business entities of a certain size, legal structure, or role in the value chain. 

Examples: Consumers, Retailers, Wholesalers, or Public Institutions"""@en .

gr:amountOfThisGood rdfs:comment "This property specifies the quantity of the goods included in the gr:Offering via this gr:TypeAndQuantityNode. The quantity is given in the unit of measurement attached to the gr:TypeAndQuantityNode."@en .

gr:TypeAndQuantityNode rdfs:comment """This class collates all the information about a gr:ProductOrService included in a bundle. If a gr:Offering contains just one item, you can directly link from the gr:Offering to the gr:ProductOrService using gr:includes. If the offering contains multiple items, use an instance of this class for each component to indicate the quantity, unit of measurement, and type of product, and link from the gr:Offering via gr:includesObject.

Example: An offering may include of 100g of Butter and 1 kg of potatoes, or 1 cell phone and 2 headsets."""@en .

gr:serialNumber rdfs:comment """The serial number or any alphanumeric identifier of a particular product. Note that serial number are unique only for the same brand or the same model, so you cannot infer from two occurrences of the same serial number that the objects to which they are attached are identical.

This property can also be attached to a gr:Offering in cases where the included products are not modeled in more detail."""@en .

gr:Individual rdfs:comment """A gr:Individual is an actual product or service instance, i.e., a single identifiable object or action that creates some increase in utility (in the economic sense) for the individual possessing or using this very object (product) or for the individual in whose favor this very action is being taken (service). Products or services are types of goods in the economic sense. For an overview of goods and commodities in economics, see Milgate (1987).

Examples: MyThinkpad T60, the pint of beer standing in front of me, my Volkswagen Golf, the haircut that I received or will be receiving at a given date and time.

Note 1: In many cases, product or service instances are not explicitly exposed on the Web but only claimed to exist (i.e. existentially quantified). In this case, use gr:SomeItems.
Note 2: This class is the new, shorter form of the former gr:ActualProductOrServiceInstance.

Compatibility with schema.org: This class is a subclass of http://schema.org/Product."""@en .

gr:hasISICv4 rdfs:comment """The International Standard of Industrial Classification of All Economic Activities (ISIC), Revision 4 code for a particular gr:BusinessEntity or gr:Location. See http://unstats.un.org/unsd/cr/registry/isic-4.asp for more information.

Note: While ISIC codes are sometimes misused for classifying products or services, they are designed and suited only for classifying business establishments."""@en .

gr:opens rdfs:comment """The opening hour of the gr:Location on the given gr:DayOfWeek.
If no time-zone suffix is included, the time is given in the local time valid at the gr:Location.

For a time in GMT/UTC, simply add a \"Z\" following the time:

09:30:10Z.

Alternatively, you can specify an offset from the UTC time by adding a positive or negative time following the time:

09:30:10-09:00

or

09:30:10+09:00.

Note 1: Use 00:00:00 for the first second of the respective day and 23:59:59 for the last second of that day.
Note 2: If a store opens at 17:00 on Saturdays and closes at 03:00:00 a.m. next morning, use 17:00:00 - 23:59:59 for Saturday and 00:00:00 - 03:00:00 for Sunday.
Note 3: If the shop re-opens on the same day of the week or set of days of the week, you must create a second instance of gr:OpeningHoursSpecification."""@en .

gr:OpeningHoursSpecification rdfs:comment "This is a conceptual entity that holds together all information about the opening hours on a given day (gr:DayOfWeek)."@en .

gr:hasNAICS rdfs:comment """The North American Industry Classification System (NAICS) code for a particular gr:BusinessEntity.
See http://www.census.gov/eos/www/naics/ for more details.

Note: While NAICS codes are sometimes misused for classifying products or services, they are designed and suited only for classifying business establishments."""@en .

gr:legalName rdfs:comment "The legal name of the gr:BusinessEntity."@en .

gr:FederalExpress rdfs:comment "Delivery via the parcel service Federal Express."@en .

gr:DeliveryModeParcelService rdfs:comment """A private parcel service as the delivery mode available for a certain offering.

Examples: UPS, DHL"""@en .

gr:hasMPN rdfs:comment """The Manufacturer Part Number or MPN is a unique identifier for a product, service, or bundle from the perspective of a particular manufacturer. MPNs can be assigned to products or product datasheets, or bundles. Accordingly, the domain of this property is the union of gr:ProductOrService (the common superclass of goods and datasheets), and gr:Offering.

Important: Be careful when assuming two products or services instances or offering instances to be identical based on the MPN. Since MPNs are unique only for the same gr:BusinessEntity, this holds only when the two MPN values refer to the same gr:BusinessEntity. Such can be done by taking into account the provenance of the data. 

Usually, the properties gr:hasEAN_UCC-13 and gr:hasGTIN-14 are much more reliable identifiers, because they are globally unique.

See also http://en.wikipedia.org/wiki/Part_number"""@en .

gr:ProductOrService rdfs:comment """The superclass of all classes describing products or services types, either by nature or purpose. Examples for such subclasses are \"TV set\", \"vacuum cleaner\", etc. An instance of this class can be either an actual product or service (gr:Individual), a placeholder instance for unknown instances of a mass-produced commodity (gr:SomeItems), or a model / prototype specification (gr:ProductOrServiceModel). When in doubt, use gr:SomeItems.

Examples: 
a) MyCellphone123, i.e. my personal, tangible cell phone (gr:Individual)
b) Siemens1234, i.e. the Siemens cell phone make and model 1234 (gr:ProductOrServiceModel)
c) dummyCellPhone123 as a placeholder for actual instances of a certain kind of cell phones (gr:SomeItems)
	
Note: Your first choice for specializations of gr:ProductOrService should be http://www.productontology.org.

Compatibility with schema.org: This class is (approximately) equivalent to http://schema.org/Product."""@en .

gr:vatID rdfs:comment "The Value-added Tax ID of the gr:BusinessEntity. See http://en.wikipedia.org/wiki/Value_added_tax_identification_number for details."@en .

gr:DHL rdfs:comment "Delivery via the parcel service DHL."@en .

gr:DeliveryModeMail rdfs:comment "Delivery via regular mail service (private or public postal services)."@en .

gr:DeliveryMethod rdfs:comment """A delivery method is a standardized procedure for transferring the product or service to the destination of fulfilment chosen by the customer. Delivery methods are characterized by the means of transportation used, and by the organization or group that is the contracting party for the sending gr:BusinessEntity (this is important, since the contracted party may subcontract the fulfilment to smaller, regional businesses).

Examples: Delivery by mail, delivery by direct download, delivery by UPS"""@en .

gr:category rdfs:comment """The name of a category to which this gr:ProductOrService, gr:Offering, gr:BusinessEntity, or gr:Location belongs.
	
Note 1: For products, it is better to add an rdf:type statement referring to a GoodRelations-compliant ontology for vertical industries instead, but if you just have a short text label, gr:category is simpler.
Note 2: You can use greater signs or slashes to informally indicate a category hierarchy, e.g. \"restaurants/asian_restaurants\" or \"cables > usb_cables\"
"""@en .

gr:hasPOS rdfs:comment "This property states that the respective gr:Location is a point of sale for the respective gr:BusinessEntity. It allows linking those two types of entities without the need for a particular gr:Offering."@en .

gr:availabilityEnds rdfs:comment """This property specifies the end of the availability of the gr:ProductOrService included in the gr:Offering.
The difference to the properties gr:validFrom and gr:validThrough is that those specify the period of time during which the offer is valid and can be accepted.

Example: I offer to lease my boat for the period of August 1 - August 31, 2010, but you must accept by offer no later than July 15.

A time-zone should be specified. For a time in GMT/UTC, simply add a \"Z\" following the time:

2008-05-30T09:30:10Z.

Alternatively, you can specify an offset from the UTC time by adding a positive or negative time following the time:

2008-05-30T09:30:10-09:00

or

2008-05-30T09:30:10+09:00.

Note: There is another property gr:availableAtOrFrom, which is used to indicate the gr:Location (e.g. store or shop) from which the goods would be available."""@en .

gr:eligibleCustomerTypes rdfs:comment "The types of customers (gr:BusinessEntityType) for which the given gr:Offering is valid."@en .

gr:ByInvoice rdfs:comment "Payment by bank transfer after delivery, i.e., the offering gr:BusinessEntity will deliver first, inform the buying party about the due amount and their bank account details, and expect payment shortly after delivery."@en .

gr:PaymentMethod rdfs:comment """A payment method is a standardized procedure for transferring the monetary amount for a purchase. Payment methods are characterized by the legal and technical structures used, and by the organization or group carrying out the transaction. This element is mostly used for specifying the types of payment accepted by a gr:BusinessEntity.

Examples: VISA, MasterCard, Diners, cash, or bank transfer in advance."""@en .

gr:hasInventoryLevel rdfs:comment """This property specifies the current approximate inventory level for gr:SomeItems. The unit of measurement and the point value or interval are indicated using the attached gr:QuantitativeValueFloat instance.

This property can also be attached to a gr:Offering in cases where the included products are not modeled in more detail."""@en .

gr:QuantitativeValueFloat rdfs:comment """An instance of this class is an actual float value for a quantitative property of a product. This instance is usually characterized by a minimal value, a maximal value, and a unit of measurement.

Examples: The intervals \"between 10.0  and 25.4 kilogramms\" or \"10.2 and 15.5 milimeters\".

Compatibility with schema.org: This class is a subclass of http://schema.org/Quantity."""@en .

gr:SomeItems rdfs:comment """A placeholder instance for unknown instances of a mass-produced commodity. This is used as a computationally cheap work-around for such instances that are not individually exposed on the Web but just stated to exist (i.e., which are existentially quantified).

Example: An instance of this class can represent an anonymous set of green Siemens1234 phones. It is different from the gr:ProductOrServiceModel Siemens1234, since this refers to the make and model, and it is different from a particular instance of this make and model (e.g. my individual phone) since the latter can be sold only once.

Note: This class is the new, shorter form of the former gr:ProductOrServicesSomeInstancesPlaceholder.
		
Compatibility with schema.org: This class is (approximately) a subclass of http://schema.org/Product."""@en .

gr:isSimilarTo rdfs:comment "This states that a given gr:ProductOrService is similar to another product or service. Of course, this is a subjective statement; when interpreting it, the trust in the origin of the statement should be taken into account."@en .

gr:Maintain rdfs:comment "This gr:BusinessFunction indicates that the gr:BusinessEntity offers (or seeks) typical maintenance tasks for the specified gr:ProductOrService. Maintenance tasks are actions that undo or compensate for wear or other deterioriation caused by regular usage, in order to restore the originally intended function of the product, or to prevent outage or malfunction."@en .

gr:BusinessFunction rdfs:comment """The business function specifies the type of activity or access (i.e., the bundle of rights) offered by the gr:BusinessEntity on the gr:ProductOrService through the gr:Offering. Typical are sell, rental or lease, maintenance or repair, manufacture / produce, recycle / dispose, engineering / construction, or installation.

Licenses and other proprietary specifications of access rights are also instances of this class.

Examples: A particular offering made by Miller Rentals Ltd. says that they (1) sell Volkswagen Golf convertibles, (2) lease out a particular Ford pick-up truck, and (3) dispose car wrecks of any make and model."""@en .

gr:hasOpeningHoursSpecification rdfs:comment "This property links a gr:Location to a gr:OpeningHoursSpecification."@en .

gr:validThrough rdfs:comment """This property specifies the end of the validity of the gr:Offering, gr:PriceSpecification, gr:License, or gr:OpeningHoursSpecification.
A time-zone should be specified. For a time in GMT/UTC, simply add a \"Z\" following the time:

2008-05-30T09:30:10Z.

Alternatively, you can specify an offset from the UTC time by adding a positive or negative time following the time:

2008-05-30T09:30:10-09:00

or
2008-05-30T09:30:10+09:00.

Note 1: If multiple contradicting instances of a gr:Offering, gr:PriceSpecification, or gr:OpeningHoursSpecification exist, it is a good heuristics to assume that
1. Information with validity information for the respective period of time ranks higher than information without validity information.
2. Among conflicting nodes both having validity information, the one with the shorter validity span ranks higher.
Note 2: For Google, attaching a gr:validThrough statement to a gr:UnitPriceSpecification is mandatory. 
"""@en .

gr:License rdfs:comment """A license is the specification of a bundle of rights that determines the type of activity or access offered by the gr:BusinessEntity on the gr:ProductOrService through the gr:Offering.
	
Licenses can be standardized (e.g. LPGL, Creative Commons, ...), vendor-specific, or individually defined for a single offer or product. Whether there is a fee for obtaining the license is specified using the gr:UnitPriceSpecification attached to the gr:Offering. Use foaf:page for linking to a document containing the license, e.g. in PDF or HTML."""@en .

gr:AmericanExpress rdfs:comment "Payment by credit or debit cards issued by the American Express network."@en .

gr:PaymentMethodCreditCard rdfs:comment """The subclass of gr:PaymentMethod represents all variants and brands of credit or debit cards as a standardized procedure for transferring the monetary amount for a purchase. It is mostly used for specifying the types of payment accepted by a gr:Business Entity.

Examples: VISA, MasterCard, or American Express."""@en .

gr:appliesToPaymentMethod rdfs:comment "This property specifies the gr:PaymentMethod to which the gr:PaymentChargeSpecification applies."@en .

gr:PaymentChargeSpecification rdfs:comment """A payment charge specification is a conceptual entity that specifies the additional costs asked for settling the payment after accepting a given gr:Offering using a particular gr:PaymentMethod. A payment charge specification is characterized by (1) a monetary amount per order specified as a literal value of type float in combination with a Currency, (2) the payment method, and (3) a whether this charge includes local sales taxes, namely VAT.
A gr:Offering may be linked to multiple payment charge specifications that specify alternative charges for various payment methods.

Examples: Payment by VISA or Mastercard costs a fee of 3 Euros including VAT, payment by bank transfer in advance is free of charge.

The total amount of this surcharge is specified as a float value of the gr:hasCurrencyValue property. The currency is specified via the gr:hasCurrency datatype property. Whether the price includes VAT or not is indicated by the gr:valueAddedTaxIncluded datatype property. The gr:PaymentMethod to which this charge applies is specified using the gr:appliesToPaymentMethod object property.

If the price can only be given as a range, use gr:hasMaxCurrencyValue and gr:hasMinCurrencyValue for the upper and lower bounds.

Important: When querying for the price, always use gr:hasMaxCurrencyValue and gr:hasMinCurrencyValue."""@en .

gr:isConsumableFor rdfs:comment "This states that a particular gr:ProductOrService is a consumable for another product or service."@en .

gr:hasValueFloat rdfs:comment "This subproperty specifies that the upper and lower limit of the given gr:QuantitativeValueFloat are identical and have the respective float value. It is a shortcut for such cases where a quantitative property is (at least practically) a single point value and not an interval."@en .

gr:hasMaxValueFloat rdfs:comment "This property captures the upper limit of a gr:QuantitativeValueFloat instance."@en .

gr:hasMaxValue rdfs:comment "This property captures the upper limit of a gr:QuantitativeValue instance."@en .

gr:hasMinValueFloat rdfs:comment "This property captures the lower limit of a gr:QuantitativeValueFloat instance."@en .

gr:hasMinValue rdfs:comment "This property captures the lower limit of a gr:QuantitativeValue instance."@en .

gr:closes rdfs:comment """The closing  hour of the gr:Location on the given gr:DayOfWeek.
If no time-zone suffix is included, the time is given in the local time valid at the gr:Location.

For a time in GMT/UTC, simply add a \"Z\" following the time:

09:30:10Z.

Alternatively, you can specify an offset from the UTC time by adding a positive or negative time following the time:

09:30:10-09:00

09:30:10+09:00.

Note 1: Use 00:00:00 for the first second of the respective day and 23:59:59 for the last second of that day.
Note 2: If a store opens at 17:00 on Saturdays and closes at 03:00:00 a.m. next morning, use two instances of this class, one with 17:00:00 - 23:59:59 for Saturday and another one with 00:00:00 - 03:00:00 for Sunday.
Note 3: If the shop re-opens on the same day of the week or set of days of the week, you must create a second instance of gr:OpeningHoursSpecification."""@en .

gr:PaySwarm rdfs:comment "Payment via the PaySwarm distributed micropayment service."@en .

gr:advanceBookingRequirement rdfs:comment """The minimal and maximal amount of time that is required between accepting the gr:Offering and the actual usage of the resource or service. This is mostly relevant for offers regarding hotel rooms, the rental of objects, or the provisioning of services. The duration is specified relatively to the beginning of the usage of the contracted object. It is represented by attaching an instance of the class gr:QuantitativeValueInteger. The lower and upper boundaries are specified using the properties gr:hasMinValueInteger and gr:hasMaxValueInteger to that instance. The unit of measurement is specified using the property gr:hasUnitOfMeasurement with a string holding a UN/CEFACT code suitable for durations, e.g. MON (months), DAY (days), HUR (hours), or MIN (minutes).

The difference to the gr:validFrom and gr:validThrough properties is that those specify the interval during which the gr:Offering is valid, while gr:advanceBookingRequirement specifies the acceptable relative amount of time between accepting the offer and the fulfilment or usage."""@en .

gr:eligibleTransactionVolume rdfs:comment """This property can be used to indicate the transaction volume, in a monetary unit, for which the gr:Offering or gr:PriceSpecification is valid. This is mostly used to specify a minimal purchasing volume, to express free shipping above a certain order volume, or to limit the acceptance of credit cards to purchases above a certain amount.

The object is a gr:PriceSpecification that uses the properties gr:hasMaxCurrencyValue and gr:hasMinCurrencyValue to indicate the lower and upper boundaries and gr:hasCurrency to indicate the currency using the ISO 4217 standard (3 characters)."""@en .

gr:durationOfWarrantyInMonths rdfs:comment "This property specifies the duration of the gr:WarrantyPromise in months."@en .

gr:WarrantyPromise rdfs:comment """This is a conceptual entity that holds together all aspects of the n-ary relation gr:hasWarrantyPromise.

A Warranty promise is an entity representing the duration and scope of services that will be provided to a customer free of charge in case of a defect or malfunction of the gr:ProductOrService. A warranty promise is characterized by its temporal duration (usually starting with the date of purchase) and its gr:WarrantyScope. The warranty scope represents the types of services provided (e.g. labor and parts, just parts) of the warranty included in an gr:Offering. The actual services may be provided by the gr:BusinessEntity making the offering, by the manufacturer of the product, or by a third party. There may be multiple warranty promises associated with a particular offering, which differ in duration and scope (e.g. pick-up service during the first 12 months, just parts and labor for 36 months).

Examples: 12 months parts and labor, 36 months parts"""@en .

gr:hasGlobalLocationNumber rdfs:comment """The Global Location Number (GLN, sometimes also referred to as International Location Number or ILN) of the respective gr:BusinessEntity or gr:Location.
The Global Location Number is a thirteen-digit number used to identify parties and physical locations."""@en .

gr:isVariantOf rdfs:comment """This states that a particular gr:ProductOrServiceModel is a variant of another product or service model. It is pretty safe to infer that the variant inherits all gr:quantitativeProductOrServiceProperty, gr:qualitativeProductOrServiceProperty, and gr:datatypeProductOrServiceProperty values that are defined for the first gr:ProductOrServiceModel.

Example:
foo:Red_Ford_T_Model gr:isVariantOf foo:Ford_T_Model"""@en .

gr:ProductOrServiceModel rdfs:comment """A product or service model is a intangible entity that specifies some characteristics of a group of similar, usually mass-produced products, in the sense of a prototype. In case of mass-produced products, there exists a relation gr:hasMakeAndModel between the actual product or service (gr:Individual or gr:SomeItems) and the prototype (gr:ProductOrServiceModel). GoodRelations treats product or service models as \"prototypes\" instead of a completely separate kind of entities, because this allows using the same domain-specific properties (e.g. gr:weight) for describing makes and models and for describing actual products.

Examples: Ford T, Volkswagen Golf, Sony Ericsson W123 cell phone

Note: An actual product or service (gr:Individual) by default shares the features of its model (e.g. the weight). However, this requires non-standard reasoning. See http://wiki.goodrelations-vocabulary.org/Axioms for respective rule sets.
	
Compatibility with schema.org: This class is (approximately) a subclass of http://schema.org/Product."""@en .

gr:hasGTIN-8 rdfs:comment "The 8-digit Global Trade Item Number (GTIN-8) of the given gr:ProductOrService or gr:Offering, also known as EAN/UCC-8 (8-digit EAN)."@en .

gr:PartsAndLabor-PickUp rdfs:comment """In case of a defect or malfunction, the buying party has the right to request from the selling gr:Business Entity to pick-up the good from its current location to a suitable service location, where the functionality of the good will be restored. All transportation, labor, parts, and materials needed to fix the problem will be covered by the selling business entity or one of its partnering business entities.
  
Note: This is just a rough classification for filtering offers. It is up to the buying party to check the exact scope and terms and conditions of the gr:WarrantyPromise."""@en .

gr:WarrantyScope rdfs:comment """The warranty scope represents types of services that will be provided free of charge by the vendor or manufacturer in the case of a defect (e.g. labor and parts, just parts), as part of the warranty included in an gr:Offering. The actual services may be provided by the gr:BusinessEntity making the offering, by the manufacturer of the product, or by a third party. 

Examples: Parts and Labor, Parts"""@en .

gr:JCB rdfs:comment "Payment by credit or debit cards issued by the JCB network."@en .

gr:depth rdfs:comment """The depth of the product.
Typical unit code(s): CMT for centimeters, INH for inches"""@en .

gr:QuantitativeValue rdfs:comment """A quantitative value is a numerical interval that represents the range of a certain gr:quantitativeProductOrServiceProperty in terms of the lower and upper bounds for a particular gr:ProductOrService. It is to be interpreted in combination with the respective unit of measurement. Most quantitative values are intervals even if they are in practice often treated as a single point value.
	
Example: a weight between 10 and 25 kilogramms, a length between 10 and 15 milimeters.

Compatibility with schema.org: This class is equivalent to http://schema.org/Quantity."""@en .

gr:quantitativeProductOrServiceProperty rdfs:comment "This is the super property of all quantitative  properties for products and services. All properties in product or service ontologies that specify quantitative characteristics, for which an interval is at least theoretically an appropriate value, are subproperties of this property."@en .

gr:hasValueInteger rdfs:comment "This subproperty specifies that the upper and lower limit of the given gr:QuantitativeValueInteger are identical and have the respective integer value. It is a shortcut for such cases where a quantitative property is (at least practically) a single point value and not an interval."@en .

gr:hasMinValueInteger rdfs:comment "This property captures the lower limit of a gr:QuantitativeValueInteger instance."@en .

gr:hasMaxValueInteger rdfs:comment "This property captures the upper limit of a gr:QuantitativeValueInteger instance."@en .

gr:hasManufacturer rdfs:comment "This object property links a gr:ProductOrService to the gr:BusinessEntity that produces it. Mostly used with gr:ProductOrServiceModel."@en .

gr:description rdfs:comment """A short textual description of the resource. 

This property is semantically equivalent to rdfs:comment and just meant as a handy shortcut for marking up data."""@en .

gr:Brand rdfs:comment """A brand is the identity of a specific product, service, or business. Use foaf:logo for attaching a brand logo and gr:name or rdfs:label for attaching the brand name.	

(Source: Wikipedia, the free encyclopedia, see http://en.wikipedia.org/wiki/Brand)"""@en .

gr:DayOfWeek rdfs:comment """The day of the week, used to specify  to which day the opening hours of a gr:OpeningHoursSpecification refer.

Examples: Monday, Tuesday, Wednesday,..."""@en .

gr:DeliveryChargeSpecification rdfs:comment """A delivery charge specification is a conceptual entity that specifies the additional costs asked for the delivery of a given gr:Offering using a particular gr:DeliveryMethod by the respective gr:BusinessEntity. A delivery charge specification is characterized by (1) a monetary amount per order, specified as a literal value of type float in combination with a currency, (2) the delivery method, (3) the target country or region, and (4)  whether this charge includes local sales taxes, namely VAT.
A gr:Offering may be linked to multiple gr:DeliveryChargeSpecification nodes that specify alternative charges for disjoint combinations of target countries or regions, and delivery methods.

Examples: Delivery by direct download is free of charge worldwide, delivery by UPS to Germany is 10 Euros per order, delivery by mail within the US is 5 Euros per order.

The total amount of this charge is specified as a float value of the gr:hasCurrencyValue property. The currency is specified via the gr:hasCurrency datatype property. Whether the price includes VAT or not is indicated by the gr:valueAddedTaxIncluded property. The gr:DeliveryMethod to which this charge applies is specified using the gr:appliesToDeliveryMethod object property. The region or regions to which this charge applies is specified using the gr:eligibleRegions property, which uses ISO 3166-1 and ISO 3166-2 codes.

If the price can only be given as a range, use gr:hasMaxCurrencyValue and gr:hasMinCurrencyValue for the upper and lower bounds.

Important: When querying for the price, always use gr:hasMaxCurrencyValue and gr:hasMinCurrencyValue."""@en .

gr:QualitativeValue rdfs:comment """A qualitative value is a predefined value for a product characteristic. 
	
Examples: the color \"green\" or the power cord plug type \"US\"; the garment sizes \"S\", \"M\", \"L\", and \"XL\".
	
Note: Value sets are supported by creating subclasses of this class. Ordinal relations between values (gr:greater, gr:lesser, ...) are provided directly by GoodRelations.

Compatibility with schema.org: This class is equivalent to http://schema.org/Enumeration."""@en .

gr:UnitPriceSpecification rdfs:comment """A unit price specification is a conceptual entity that specifies the price asked for a given gr:Offering by the respective gr:Business Entity. An offering may be linked to multiple unit price specifications that specify alternative prices for non-overlapping sets of conditions (e.g. quantities or sales regions) or with differing validity periods. 

A unit price specification is characterized by (1) the lower and upper limits and the unit of measurement of the eligible quantity, (2) by a monetary amount per unit of the product or service, and (3)  whether this prices includes local sales taxes, namely VAT.
	
Example: The price, including VAT, for 1 kg of a given material is 5 Euros per kg for 0 - 5 kg and 4 Euros for quantities above 5 kg.

The eligible quantity interval for a given price is specified using the object property gr:hasEligibleQuantity, which points to an instance of gr:QuantitativeValue. The currency is specified using the gr:hasCurrency property, which points to an ISO 4217 currency code. The unit of measurement for the eligible quantity is specified using the gr:hasUnitOfMeasurement datatype property, which points to an UN/CEFACT Common Code (3 characters).
	
In most cases, the appropriate unit of measurement is the UN/CEFACT Common Code \"C62\" for \"Unit or piece\", since a gr:Offering is defined by the quantity and unit of measurement of all items included (e.g. \"1 kg of bananas plus a 2 kg of apples\"). As long at the offering consists of only one item, it is also possible to use an unit of measurement of choice for specifying the price per unit. For bundles, however, only  \"C62\" for \"Unit or piece\" is a valid unit of measurement.

You can assume that the price is given per unit or piece if there is no gr:hasUnitOfMeasurement property attached to the price.
	
Whether VAT and sales taxes are included in this price is specified using the property gr:valueAddedTaxIncluded (xsd:boolean).
	
The price per unit of measurement is specified as a float value of the gr:hasCurrencyValue property. The currency is specified via the gr:hasCurrency datatype property. Whether the price includes VAT or not is indicated by the gr:valueAddedTaxIncluded datatype property.

The property priceType can be used to indicate that the price is a retail price recommendation only (i.e. a list price). 

If the price can only be given as a range, use gr:hasMaxCurrencyValue and gr:hasMinCurrencyValue for the upper and lower bounds.

Important: When querying for the price, always use gr:hasMaxCurrencyValue and gr:hasMinCurrencyValue.

Note 1: Due to the complexity of pricing scenarios in various industries, it may be necessary to create extensions of this fundamental model of price specifications. Such can be done easily by importing and refining the GoodRelations ontology.

Note 2: For Google, attaching a gr:validThrough statement to a gr:UnitPriceSpecification is mandatory. 
"""@en .

gr:Cash rdfs:comment "Payment by cash upon delivery or pickup."@en .

gr:DinersClub rdfs:comment "Payment by credit or debit cards issued by the Diner's Club network."@en .

gr:Dispose rdfs:comment "This gr:BusinessFunction indicates that the gr:BusinessEntity offers (or seeks) the acceptance of the specified gr:ProductOrService for proper disposal, recycling, or any other kind of allowed usages, freeing the current owner from all rights and obligations of ownership."@en .

gr:billingIncrement rdfs:comment """This property specifies the minimal quantity and rounding increment that will be the basis for the billing. 
The unit of measurement is specified by the UN/CEFACT code attached to the gr:UnitPriceSpecification via the gr:hasUnitOfMeasurement property.

Examples: 
- The price for gasoline is 4 USD per gallon at the pump, but you will be charged in units of 0.1 gallons.
- The price for legal consulting is 100 USD per hour, but you will be charged in units of 15 minutes.

This property makes sense only for instances of gr:Offering that include not more than one type of good or service."""@en .

gr:isListPrice rdfs:comment """This boolean attribute indicates whether a gr:UnitPriceSpecification is a list price (usually a vendor recommendation) or not. \"true\"  indicates it is a list price, \"false\" indicates it is not.
DEPRECATED. Use the gr:priceType property instead."""@en .

gr:color rdfs:comment "The color of the product."@en .

gr:datatypeProductOrServiceProperty rdfs:comment """This property is the super property for all pure datatype properties that can be used to describe a gr:ProductOrService.

In products and services ontologies, only such properties that are no quantitative properties and that have no predefined gr:QualitativeValue instances are subproperties of this property. In practice, this refers to a few integer properties for which the integer value represents qualitative aspects, for string datatypes (as long as no predefined values exist), for boolean datatype properties, and for dates and times."""@en .

gr:isAccessoryOrSparePartFor rdfs:comment "This states that a particular gr:ProductOrService is an accessory or spare part for another product or service."@en .

gr:hasDUNS rdfs:comment "The Dun & Bradstreet DUNS number for identifying a gr:BusinessEntity. The Dun & Bradstreet DUNS is a nine-digit number used to identify legal entities (but usually not branches or locations of logistical importance only)."@en .

gr:typeOfGood rdfs:comment "This specifies the gr:ProductOrService that the gr:TypeAndQuantityNode is referring to."@en .

gr:deliveryLeadTime rdfs:comment """This property can be used to indicate the promised delay between the receipt of the order and the goods leaving the warehouse.

The duration is specified by attaching an instance of gr:QuantitativeValueInteger. The lower and upper boundaries are specified using the properties gr:hasMinValueInteger and gr:hasMaxValueInteger to that instance. A point value can be modeled with the gr:hasValueInteger property. The unit of measurement is specified using the property gr:hasUnitOfMeasurement with a string holding a UN/CEFACT code suitable for durations, e.g. MON (months), DAY (days), HUR (hours), or MIN (minutes)."""@en .

gr:hasStockKeepingUnit rdfs:comment """The Stock Keeping Unit, or SKU is a unique identifier for a product, service, or bundle from the perspective of a particular supplier, i.e. SKUs are mostly assigned and serialized at the merchant level. 
Examples of SKUs are the ordering or parts numbers used by a particular Web shop or catalog.

Consequently, the domain of gr:hasStockKeepingUnit is the union of the classes gr:Offering and gr:ProductOrService. 
If attached to a gr:Offering, the SKU will usually reflect a merchant-specific identifier, i.e. one valid only for that particular retailer or shop. 
If attached to a gr:ProductOrServiceModel, the SKU can reflect either the identifier used by the merchant or the part number used by the official manufacturer of that part. For the latter, gr:hasMPN is a better choice.

Important: Be careful when assuming two products or services instances or offering instances to be identical based on the SKU. Since SKUs are unique only for the same gr:BusinessEntity, this can be assumed only when you are sure that the two SKU values refer to the same business entity. Such can be done by taking into account the provenance of the data. As long as instances of gr:Offering are concerned, you can also check that the offerings are being offered by the same gr:Business Entity.

Usually, the properties gr:hasEAN_UCC-13 and gr:hasGTIN-14 are much more reliable identifiers, because they are globally unique.

See also http://en.wikipedia.org/wiki/Stock_Keeping_Unit."""@en .

gr:qualitativeProductOrServiceProperty rdfs:comment "This is the super property of all qualitative properties for products and services. All properties in product or service ontologies for which gr:QualitativeValue instances are specified are subproperties of this property."@en .

gr:availableDeliveryMethods rdfs:comment "This specifies the gr:DeliveryMethod or methods available for a given gr:Offering."@en .

gr:Repair rdfs:comment "This gr:BusinessFunction indicates that the gr:BusinessEntity offers (or seeks) the evaluation of the chances for repairing, and, if positive, repair of the specified gr:ProductOrService. Repairing means actions that restore the originally intended function of a product that suffers from outage or malfunction."@en .

gr:GoogleCheckout rdfs:comment "Payment via the Google Checkout payment service."@en .

gr:includes rdfs:comment """This object property is a shortcut for the original gr:includesObject property for the common case of having exactly one single gr:ProductOrService instance included in an Offering. 

When linking to an instance of gr:SomeItems or gr:Individual, it is equivalent to using a gr:TypeAndQuantityNode with gr:hasUnitOfMeasurement=\"C62\"^^xsd:string and gr:amountOfThisGood=\"1.0\"^^xsd:float for that good.

When linking to a gr:ProductOrServiceModel, it is equivalent to 
1. defining an blank node for a gr:SomeItems
2. linking that blank node via gr:hasMakeAndModel to the gr:ProductOrServiceModel, and
3. linking from the gr:Offering to that blank node using another blank node of type gr:TypeAndQuantityNode with gr:hasUnitOfMeasurement=\"C62\"^^xsd:string and gr:amountOfThisGood=\"1.0\"^^xsd:float for that good."""@en .

gr:Business rdfs:comment "The gr:BusinessEntityType representing such agents that are themselves offering commercial services or products on the market. Usually, businesses are characterized by the fact that they are officially registered with the public administration and strive for profits by their activities."@en .

gr:Sell rdfs:comment "This gr:BusinessFunction indicates that the gr:BusinessEntity offers to permanently transfer all property rights on the specified gr:ProductOrService."@en .

gr:hasValue rdfs:comment "This subproperty specifies that the upper and lower limit of the given gr:QuantitativeValue are identical and have the respective value. It is a shortcut for such cases where a quantitative property is (at least practically) a single point value and not an interval."@en .

gr:hasBrand rdfs:comment "This specifies the brand or brands (gr:Brand) associated with a gr:ProductOrService, or the brand or brands maintained by a gr:BusinessEntity."@en .

gr:ByBankTransferInAdvance rdfs:comment """Payment by bank transfer in advance, i.e., the offering gr:BusinessEntity will inform the buying party about their bank account details and will deliver the goods upon receipt of the due amount.
This is equivalent to payment by wire transfer."""@en .

gr:hasOpeningHoursDayOfWeek rdfs:comment """This specifies the gr:DayOfWeek to which the gr:OpeningHoursSpecification is related.

Note: Use multiple instances of gr:OpeningHoursSpecification for specifying the opening hours for multiple days if the opening hours differ."""@en .

gr:priceType rdfs:comment """This attribute can be used to distinguish multiple different price specifications for the same gr:Offering. It supersedes the former gr:isListPrice property. The following values are recommended:

The absence of this property marks the actual sales price.

SRP: \"suggested retail price\" - applicable for all sorts of a non-binding retail price recommendations, e.g. such published by the manufacturer or the distributor. This value replaces the former gr:isListPrice property.

INVOICE: The invoice price, mostly used in the car industry - this is the price a dealer pays to the manufacturer, excluding rebates and charges."""@en .

gr:DeliveryModeOwnFleet rdfs:comment "Delivery of the goods by using a fleet of vehicles either owned and operated or subcontracted by the gr:BusinessEntity."@en .

gr:eligibleRegions rdfs:comment """This property specifies the geo-political region or regions for which the gr:Offering, gr:License, or gr:DeliveryChargeSpecification is valid using the two-character version of ISO 3166-1 (ISO 3166-1 alpha-2)  for regions or ISO 3166-2 , which breaks down the countries from ISO 3166-1 into administrative subdivisions.

Important: Do NOT use 3-letter ISO 3166-1 codes!"""@en .

gr:VISA rdfs:comment "Payment by credit or debit cards issued by the VISA network."@en .

gr:valueReference rdfs:comment "The superclass of properties that link a gr:QuantitativeValue or a gr:QualitativeValue to a second gr:QuantitativeValue or a gr:QualitativeValue that provides additional information on the original value. A good modeling practice is to define specializations of this property (e.g. foo:referenceTemperature) for your particular domain."@en .

gr:validFrom rdfs:comment """This property specifies the beginning of the validity of the gr:Offering, gr:PriceSpecification, gr:License, or gr:OpeningHoursSpecification.
A time-zone should be specified. For a time in GMT/UTC, simply add a \"Z\" following the time:

2008-05-30T09:30:10Z.

Alternatively, you can specify an offset from the UTC time by adding a positive or negative time following the time:

2008-05-30T09:30:10-09:00

or

2008-05-30T09:30:10+09:00.

Note: If multiple contradicting instances of a gr:Offering, gr:PriceSpecification, or gr:OpeningHoursSpecification exist, it is a good heuristics to assume that
1. Information with validity information for the respective period of time ranks higher than information without validity information.
2. Among conflicting nodes both having validity information, the one with the shorter validity span ranks higher."""@en .

gr:DeliveryModeDirectDownload rdfs:comment "Delivery of the goods via direct download from the Internet, i.e., the offering gr:BusinessEntity provides the buying party with details on how to retrieve the goods online. Connection fees and other costs of using the infrastructure are to be carried by the buying party."@en .

gr:UPS rdfs:comment "Delivery via the parcel service UPS."@en .

gr:ConstructionInstallation rdfs:comment "This gr:BusinessFunction indicates that the gr:BusinessEntity offers (or seeks) the construction and/or installation of the specified gr:ProductOrService at the customer's location."@en .

gr:CheckInAdvance rdfs:comment "Payment by sending a check in advance, i.e., the offering gr:BusinessEntity will deliver the goods upon receipt of a check over the due amount. There are variations in handling payment by check - sometimes, shipment will be upon receipt of the check as a document, sometimes the shipment will take place only upon successful crediting of the check."@en .

gr:name rdfs:comment """A short text describing the respective resource.

This property is semantically equivalent to dcterms:title and rdfs:label and just meant as a handy shortcut for marking up data."""@en .

gr:hasWarrantyPromise rdfs:comment "This specifies the gr:WarrantyPromise made by the gr:BusinessEntity for the given gr:Offering."@en .

gr:hasGTIN-14 rdfs:comment "The Global Trade Item Number (GTIN-14) of the given gr:ProductOrService or gr:Offering."@en .

gr:LeaseOut rdfs:comment "This gr:BusinessFunction indicates that the gr:BusinessEntity offers (or seeks) the temporary right to use the specified gr:ProductOrService."@en .

gr:hasCurrencyValue rdfs:comment """This property specifies the amount of money for a price per unit, shipping charges, or payment charges. The currency and other relevant details are attached to the respective gr:PriceSpecification etc.

For a gr:UnitPriceSpecification, this is the price for one unit or bundle (as specified in the unit of measurement of the unit price specification) of the respective gr:ProductOrService. For a gr:DeliveryChargeSpecification or a gr:PaymentChargeSpecification, it is the price per delivery or payment.

GoodRelations also supports giving price information as intervals only. If this is needed, use gr:hasMaxCurrencyValue for the upper bound and gr:hasMinCurrencyValue for the lower bound. 

Using gr:hasCurrencyValue sets the upper and lower bounds to the same given value, i.e., x gr:hasCurrencyValue y implies x gr:hasMinCurrencyValue y, x gr:hasMaxCurrencyValue y."""@en .

gr:hasMinCurrencyValue rdfs:comment """This property specifies the LOWER BOUND of the amount of money for a price RANGE per unit, shipping charges, or payment charges. The currency and other relevant details are attached to the respective gr:PriceSpecification etc.
For a gr:UnitPriceSpecification, this is the LOWER BOUND for the price for one unit or bundle (as specified in the unit of measurement of the unit price specification) of the respective gr:ProductOrService. For a gr:DeliveryChargeSpecification or a gr:PaymentChargeSpecification, it is the LOWER BOUND of the price per delivery or payment.

Using gr:hasCurrencyValue sets the upper and lower bounds to the same given value, i.e., x gr:hasCurrencyValue y implies x gr:hasMinCurrencyValue y, x gr:hasMaxCurrencyValue y."""@en .

gr:hasMaxCurrencyValue rdfs:comment """This property specifies the UPPER BOUND of the amount of money for a price RANGE per unit, shipping charges, or payment charges. The currency and other relevant details are attached to the respective gr:PriceSpecification etc.
For a gr:UnitPriceSpecification, this is the UPPER BOUND for the price for one unit or bundle (as specified in the unit of measurement of the unit price specification) of the respective gr:ProductOrService. For a gr:DeliveryChargeSpecification or a gr:PaymentChargeSpecification, it is the UPPER BOUND of the price per delivery or payment.

Using gr:hasCurrencyValue sets the upper and lower bounds to the same given value, i.e., x gr:hasCurrencyValue y implies x gr:hasMinCurrencyValue y, x gr:hasMaxCurrencyValue y."""@en .

gr:hasCurrency rdfs:comment "The currency for all prices in the gr:PriceSpecification given using the ISO 4217 standard (3 characters)."@en .

gr:Buy rdfs:comment """This gr:BusinessFunction indicates that the gr:BusinessEntity is in general interested in purchasing the specified gr:ProductOrService.
DEPRECATED. Use gr:seeks instead."""@en .

gr:hasMakeAndModel rdfs:comment """This states that an actual product instance (gr:Individual) or a placeholder instance for multiple, unidentified such instances (gr:SomeItems) is one occurence of a particular gr:ProductOrServiceModel.

Example: myFordT hasMakeAndModel FordT."""@en .

gr:PartsAndLabor-BringIn rdfs:comment """In case of a defect or malfunction, the buying party has the right to transport the good to a service location determined by the the selling gr:BusinessEntity and will not be be charged for labor, parts, and materials needed to fix the problem. All those costs will be covered by the selling business entity or one of its partnering business entities.

Note: This is just a rough classification for filtering offers. It is up to the buying party to check the exact scope and terms and conditions of the gr:WarrantyPromise."""@en .

gr:Enduser rdfs:comment "The gr:BusinessEntityType representing such agents that are purchasing the good or service for private consumption, in particular not for resale or for usage within an industrial enterprise. By default, a Business Entity is an Enduser."@en .

gr:relatedWebService rdfs:comment """The URI of a SOAP or REST Web Service from which additional information about the gr:BusinessEntity, gr:Offering, gr:PriceSpecification, or gr:ProductOrService, or any other element,  can be obtained. The recommended range is xsd:anyURI i.e., the URI of a SOAP or REST Web Service.

In principle, any existing or upcoming vocabulary for Web Services can be used in combination with GoodRelations, because the association between (a) the service description and (b) the GoodRelations description can be found via the Web Service URI value used with this gr:relatedWebService property."""@en .

gr:PublicHolidays rdfs:comment "A placeholder for all official public holidays at the gr:Location. This allows specifying the opening hours on public holidays. If a given day is a public holiday, this specification supersedes the opening hours for the respective day of the week."@en .

gr:displayPosition rdfs:comment """The position at which the option or element should be listed in a menu or user dialog, lower numbers come first.

The main usage of this property are the days of the week (gr:DayOfWeek), but it is also possible to apply it e.g. to product features or any other conceptual element.
Note: Rely on this property only for data originating from a single RDF graph; otherwise, unpredictable results are possible."""@en .

gr:valueAddedTaxIncluded rdfs:comment """This property specifies whether the applicable value-added tax (VAT)  is included in the price of the gr:PriceSpecification or not.

Note: This is a simple representation which may not properly reflect all details of local taxation."""@en .

gr:acceptedPaymentMethods rdfs:comment "The gr:PaymentMethod or methods accepted by the gr:BusinessEntity for the given gr:Offering."@en .

gr:hasBusinessFunction rdfs:comment """This specifies the business function of the gr:Offering, i.e. whether the gr:BusinessEntity is offering to sell, to lease, or to repair the particular type of product. In the case of bundles, it is also possible to attach individual business functions to each gr:TypeAndQuantityNode. The business function of the main gr:Offering determines the business function for all included objects or services, unless a business function attached to a gr:TypeAndQuantityNode overrides it.
	
Note: While it is possible that an entity is offering multiple types of business functions for the same set of objects (e.g. rental and sales), this should usually not be stated by attaching multiple business functions to the same gr:Offering, since the gr:UnitPriceSpecification for the varying business functions will typically be very different."""@en .

gr:hasWarrantyScope rdfs:comment "This states the gr:WarrantyScope of a given gr:WarrantyPromise."@en .

gr:weight rdfs:comment """The weight of the gr:ProductOrService.
Typical unit code(s): GRM for gram, KGM for kilogram, LBR for pound"""@en .

gr:includesObject rdfs:comment "This object property links a gr:Offering to one or multiple gr:TypeAndQuantityNode or nodes that specify the components that are included in the respective offer."@en .

gr:hasEAN_UCC-13 rdfs:comment """The EAN·UCC-13 code of the given gr:ProductOrService or gr:Offering. This code is now officially called GTIN-13 (Global Trade Identifier Number) or EAN·UCC-13. Former 12-digit UPC codes can be converted into EAN·UCC-13 code by simply adding a preceeding zero.

Note 1: When using this property for searching by 12-digit UPC codes, you must add a preceeding zero digit.
Note 2: As of January 1, 2007, the former ISBN numbers for books etc. have been integrated into the EAN·UCC-13 code. For each old ISBN-10 code, there exists a proper translation into EAN·UCC-13 by adding \"978\" or \"979\" as prefix. Since the old ISBN-10 is now deprecated, GoodRelations does not provide a property for ISBNs."""@en .

gr:N-Ary-Relations rdfs:comment """This is the superclass for all classes that are placeholders for n-ary relations, which OWL cannot represent.
DEPRECATED. Do not use this class in data or queries."""@en .

gr:equal rdfs:comment "This ordering relation for qualitative values indicates that the subject is equal to the object."@en .

gr:Labor-BringIn rdfs:comment """In case of a defect or malfunction, the buying party has the right to transport the good to a service location determined by the the selling gr:BusinessEntity and will be charged only for parts and materials needed to fix the problem. Labor will be covered by the selling business entity or one of its partnering business entities.

Note: This is just a rough classification for filtering offers. It is up to the buying party to check the exact scope and terms and conditions of the gr:WarrantyPromise."""@en .

gr:height rdfs:comment """The height of the product.
Typical unit code(s): CMT for centimeters, INH for inches"""@en .

gr:width rdfs:comment """The width of the gr:ProductOrService.
Typical unit code(s): CMT for centimeters, INH for inches"""@en .

gr:COD rdfs:comment "Collect on delivery / Cash on delivery - A payment method where the recipient of goods pays at the time of delivery. Usually, the amount of money is collected by the transportation company handling the goods."@en .

gr:hasEligibleQuantity rdfs:comment """This specifies the interval and unit of measurement of ordering quantities for which the gr:Offering or gr:PriceSpecification is valid. This allows e.g. specifying that a certain freight charge is valid only for a certain quantity.
Note that if an offering is a bundle, i.e. it consists of more than one unit of a single type of good, or if the unit of measurement for the good is different from unit (Common Code C62), then gr:hasEligibleQuantity refers to units of this bundle. In other words, \"C62\" for \"Units or pieces\" is usually the appropriate unit of measurement."""@en .

gr:DeliveryModeFreight rdfs:comment "Delivery by an unspecified air, sea, or ground freight carrier or cargo company."@en .

gr:eligibleDuration rdfs:comment """The minimal and maximal duration for which the given gr:Offering or gr:License is valid. This is mostly used for offers regarding accommodation, the rental of objects, or software licenses. The duration is specified by attaching an instance of gr:QuantitativeValue. The lower and upper boundaries are specified using the properties gr:hasMinValue and gr:hasMaxValue to that instance. If they are the same, use the gr:hasValue property. The unit of measurement is specified using the property gr:hasUnitOfMeasurement with a string holding a UN/CEFACT code suitable for durations, e.g. MON (months), DAY (days), HUR (hours), or MIN (minutes).

The difference to the gr:validFrom and gr:validThrough properties is that those specify the absiolute interval during which the gr:Offering or gr:License is valid, while gr:eligibleDuration specifies the acceptable duration of the contract or usage."""@en .

gr:PayPal rdfs:comment "Payment via the PayPal payment service."@en .

gr:nonEqual rdfs:comment "This ordering relation for gr:QualitativeValue pairs indicates that the subject is not equal to the object."@en .

gr:condition rdfs:comment "A textual description of the condition of the product or service, or the products or services included in the offer (when attached to a gr:Offering)"@en .

gr:PublicInstitution rdfs:comment "The gr:BusinessEntityType representing such agents that are part of the adminstration or owned by the public."@en .

gr:DeliveryModePickUp rdfs:comment "Delivery of the goods by picking them up at one of the stores etc. (gr:Location) during the opening hours as specified by respective instances of gr:OpeningHoursSpecification."@en .

gr:Discover rdfs:comment "Payment by credit or debit cards issued by the Discover network."@en .

gr:DirectDebit rdfs:comment "Payment by direct debit, i.e., the buying party will inform the offering gr:BusinessEntity about its bank account details and authorizes the gr:BusinessEntity to collect the agreed amount directly from that account."@en .

gr:ProvideService rdfs:comment """This gr:BusinessFunction indicates that the gr:BusinessEntity offers (or seeks) the respective type of service.

Note: Maintain and Repair are also types of Services. However, products and services ontologies often provide classes for tangible products as well as for types of services. The business function gr:ProvideService is to be used with such goods that are services, while gr:Maintain and gr:Repair can be used with goods for which only the class of product exists in the ontology, but not the respective type of service.

Example: Car maintenance could be expressed both as \"provide the service car maintenance\" or \"maintain cars\"."""@en .

gr:appliesToDeliveryMethod rdfs:comment "This property specifies the gr:DeliveryMethod to which the gr:DeliveryChargeSpecification applies."@en .

gr:owns rdfs:comment """This property indicates that a particular person or business owns a particular product. It can be used to expose the products in one's posession in order to empower recommender systems to suggest matching offers.

Note that the product must be an instance of the class gr:Individual.

This property can also be safely applied to foaf:Agent instances."""@en .

gr:MasterCard rdfs:comment "Payment by credit or debit cards issued by the MasterCard network."@en .

gr:hasUnitOfMeasurement rdfs:comment "The unit of measurement for a gr:QuantitativeValue, a gr:UnitPriceSpecification, or a gr:TypeAndQuantityNode given using the UN/CEFACT Common Code (3 characters)."@en .

gr:offers rdfs:comment "This links a gr:BusinessEntity to the offers (gr:Offering) it makes. If you want to express interest in receiving offers, use gr:seeks instead."@en .

gr:addOn rdfs:comment "This property points from a gr:Offering to additional offerings that can only be obtained in combination with the first offering. This can be used to model supplements and extensions that are available for a surcharge. Any gr:PriceSpecification attached to the secondary offering is to be understood as an additional charge."@en .

gr:Wednesday rdfs:comment "Wednesday as a day of the week."@en .

gr:hasNext rdfs:comment """This ordering relation for gr:DayOfWeek indicates that the subject is directly followed by the object.

Example: Monday hasNext Tuesday

Since days of the week are a cycle, this property is not transitive."""@en .

gr:Thursday rdfs:comment "Thursday as a day of the week."@en .

gr:Friday rdfs:comment "Friday as a day of the week."@en .

gr:hasPrevious rdfs:comment """This ordering relation for gr:DayOfWeek indicates that the subject is directly preceeded by the object.

Example: Tuesday hasPrevious Monday

Since days of the week are a cycle, this property is not transitive."""@en .

gr:Tuesday rdfs:comment "Tuesday as a day of the week."@en .

gr:Monday rdfs:comment "Monday as a day of the week."@en .

gr:lesser rdfs:comment "This ordering relation for gr:QualitativeValue pairs indicates that the subject is lesser than the object."@en .

gr:greater rdfs:comment "This ordering relation for qualitative values indicates that the subject is greater than the object."@en .

gr:LocationOfSalesOrServiceProvisioning rdfs:comment "DEPRECATED - This class is superseded by gr:Location. Replace all occurrences of gr:LocationOfSalesOrServiceProvisioning by gr:Location, if possible."@en .

gr:ProductOrServicesSomeInstancesPlaceholder rdfs:comment "DEPRECATED - This class is superseded by gr:SomeItems. Replace all occurrences of gr:ProductOrServicesSomeInstancesPlaceholder by gr:SomeItems, if possible."@en .

gr:predecessorOf rdfs:comment """This property indicates that the subject is a previous, often discontinued variant of the gr:ProductOrServiceModel used as the object.

Example: Golf III predecessorOf Golf IV

This relation is transitive."""@en .

gr:successorOf rdfs:comment """This property indicates that the subject is a newer, often updated or improved variant of the gr:ProductOrServiceModel used as the object.

Example: Golf III successorOf Golf II

This relation is transitive."""@en .

gr:Sunday rdfs:comment "Sunday as a day of the week."@en .

gr:Saturday rdfs:comment "Saturday as a day of the week."@en .

gr:ActualProductOrServiceInstance rdfs:comment "DEPRECATED - This class is superseded by gr:Individual. Replace all occurrences of gr:ActualProductOrServiceInstance by gr:Individual, if possible."@en .

gr:greaterOrEqual rdfs:comment "This ordering relation for qualitative values indicates that the subject is greater than or equal to the object."@en .

gr:lesserOrEqual rdfs:comment "This ordering relation for gr:QualitativeValue pairs indicates that the subject is lesser than or equal to the object."@en .

pc:Contract rdfs:label "Veřejná zakázka"@cs, "Public contract"@en .

pc:FrameworkAgreement rdfs:label "Rámcová smlouva"@cs, "Framework agreement"@en .

pc:Tender rdfs:label "Nabídka"@cs, "Tender"@en .

gr:Offering rdfs:label "Offering"@en .

pc:AwardCriteriaCombination rdfs:label "Kombinace kritérií pro hodnocení dodaných nabídek"@cs,
    "Combination of contract award criteria"@en .

pc:CriterionWeighting rdfs:label "Vážené kritérium pro udělení zakázky"@cs, "Contract award weighted criterion"@en .

pc:TendersOpening rdfs:label "Tenders' opening"@en, "Otevírání nabídek"@cs .

pc:awardDate rdfs:label "Datum přidělení zakázky"@cs, "Date of contract award"@en .

pc:contact rdfs:label "Kontaktní osoba"@cs, "Contact person"@en .

pc:kind rdfs:label "Kategorie zakázky"@cs, "Contract kind"@en .

pc:procedureType rdfs:label "Druh řízení"@cs, "Procedure type"@en .

pc:contractingAuthority rdfs:label "Zadavatel"@cs, "Contracting authority"@en .

gr:BusinessEntity rdfs:label "Business entity"@en .

pc:mainObject rdfs:label "Hlavní předmět zakázky"@cs, "Main object of contract"@en .

pc:additionalObject rdfs:label "Další předmět zakázky"@cs, "Additional object of contract"@en .

pc:location rdfs:label "Místo uskutečnění zakázky"@cs, "Place of contract's realization"@en .

pc:contractPrice rdfs:label "Cena"@cs, "Price"@en .

gr:PriceSpecification rdfs:label "Price specification"@en .

pc:documentationPrice rdfs:label "Cena zadávací dokumentace k zakázce"@cs, "Price of documentation for public contract"@en .

pc:estimatedPrice rdfs:label "Odhadovaná cena zakázky"@cs, "Exact estimated price"@en .

pc:tenderDeadline rdfs:label "Lhůta pro doručení nabídek nebo přijetí žádostí o účast"@cs,
    "Time-limit for receipt of tenders or requests to participate"@en .

pc:documentationRequestDeadline rdfs:label "Lhůta pro vyžádání dokumentace k veřejné zakázce"@cs,
    "Time-limit for receipt of requests for documentation"@en .

pc:duration rdfs:label "Doba trvání zakázky"@cs, "Duration of contract"@en .

pc:tenderMaintenanceDuration rdfs:label "Doba trvání nabídky"@cs, "Duration of tender validity"@en .

pc:startDate rdfs:label "Datum začátku realizace zakázky"@cs, "Start date of contract"@en .

pc:estimatedEndDate rdfs:label "Očekávané datum konce realizace zakázky"@cs, "Estimated end date of contract"@en .

pc:actualEndDate rdfs:label "Skutečné datum konce realizace zakázky"@cs, "Actual end date of contract realization"@en .

pc:awardCriteriaCombination rdfs:label "Kombinace kritérií pro hodnocení nabídek zájemců o zakázku."@cs,
    "Criteria combination for tender evaluation."@en .

pc:lot rdfs:label "Část zakázky"@cs, "Contract lot"@en .

pc:frameworkAgreement rdfs:label "Na základě rámcové smlouvy"@cs, "On the base of a framework agreement"@en .

pc:numberOfTenders rdfs:label "Počet obdržených nabídek"@cs, "Number of tenders received"@en .

pc:tender rdfs:label "Nabídka"@cs, "Tender"@en .

pc:awardedTender rdfs:label "Vybraná nabídka"@cs, "Awarded tender"@en .

pc:subsidy rdfs:label "Dotace použitá pro zakázku"@cs, "Subsidy supplemented for contract"@en .

pc:agreedPrice rdfs:label "Smluvní cena"@cs, "Agreed price"@en .

pc:actualPrice rdfs:label "Skutečná cena po realizaci zakázky"@cs, "Actual price after contract realization"@en .

pc:attachment rdfs:label "Příloha k zakázce"@cs, "Contract attachment"@en .

pc:specification rdfs:label "Zadávací dokumentace zakázky"@cs, "Contract specification"@en .

pc:agreement rdfs:label "Smlouva na veřejnou zakázku"@cs, "Contract agreement"@en .

pc:awardCriterion rdfs:label "Kritérium pro zadání zakázky."@cs, "Criterion for contract award."@en,
    "Critères d'attribution"@fr, "Vergabekriterien"@de .

pc:expectedNumberOfOperators rdfs:label "Očekávaný počet účastníků rámcové smlouvy"@cs,
    "Expected number of operators of framework agreement"@en .

gr:QuantitativeValueInteger rdfs:label "Quantitative value integer"@en .

pc:profile rdfs:label "Profilová stránka zadavatele"@cs, "Profile web site of contracting authority"@en .

pc:authorityKind rdfs:label "Druh zadavatele"@cs, "Kind of contracting authority"@en .

pc:mainActivity rdfs:label "Hlavní aktivita"@cs, "Main activity"@en .

pc:offeredPrice rdfs:label "Nabídnutá cena v nabídce"@cs, "Offered price in tender"@en .

gr:hasPriceSpecification rdfs:label "has price specification (0..*)"@en .

pc:bidder rdfs:label "Zájemce o zakázku"@cs, "Tender bidder"@en .

pc:contract rdfs:label "Veřejná zakázka"@cs, "Public contract"@en .

pc:weightedCriterion rdfs:label "Vážené kritérium"@cs, "Weighted criterion"@en .

pc:criterionWeight rdfs:label "Váha kritéria pro výběr dodavatele zakázky"@cs, "Contract award criterion weight"@en .

gr:availabilityStarts rdfs:label "availability starts (0..1)"@en .

<http://purl.org/goodrelations/v1> rdfs:label "GoodRelations Ontology"@en .

gr:availableAtOrFrom rdfs:label "available at or from (0..*)"@en .

gr:Location rdfs:label "Location"@en .

gr:taxID rdfs:label "Tax ID (0..1)"@en .

gr:seeks rdfs:label "seeks (0..*)"@en .

gr:Reseller rdfs:label "Reseller (business entity type)"@en .

gr:BusinessEntityType rdfs:label "Business entity type"@en .

gr:amountOfThisGood rdfs:label "amount of this good (1..1)"@en .

gr:TypeAndQuantityNode rdfs:label "Type and quantity node"@en .

gr:serialNumber rdfs:label "serial number (0..*)"@en .

gr:Individual rdfs:label "Individual"@en .

gr:hasISICv4 rdfs:label "has ISIC v4 (0..*)"@en .

gr:opens rdfs:label "opens (1..1)"@en .

gr:OpeningHoursSpecification rdfs:label "Opening hours specification"@en .

gr:hasNAICS rdfs:label "has NAICS (0..*)"@en .

gr:legalName rdfs:label "legal name (0..1)"@en .

gr:FederalExpress rdfs:label "Federal Express (delivery method)"@en .

gr:DeliveryModeParcelService rdfs:label "Delivery mode parcel service"@en .

gr:hasMPN rdfs:label "has MPN (0..*)"@en .

gr:ProductOrService rdfs:label "Product or service"@en .

gr:vatID rdfs:label "VAT ID (0..1)"@en .

gr:DHL rdfs:label "DHL (delivery method)"@en .

gr:DeliveryModeMail rdfs:label "Delivery mode mail (delivery method)"@en .

gr:DeliveryMethod rdfs:label "Delivery method"@en .

gr:category rdfs:label "category (0..*)"@en .

gr:hasPOS rdfs:label "has POS (0..*)"@en .

gr:availabilityEnds rdfs:label "availability ends (0..1)"@en .

gr:eligibleCustomerTypes rdfs:label "eligible customer types (0..*)"@en .

gr:ByInvoice rdfs:label "By invoice (payment method)"@en .

gr:PaymentMethod rdfs:label "Payment method"@en .

gr:hasInventoryLevel rdfs:label "has inventory level (0..1)"@en .

gr:QuantitativeValueFloat rdfs:label "Quantitative value float"@en .

gr:SomeItems rdfs:label "Some items"@en .

gr:isSimilarTo rdfs:label "is similar to (0..*)"@en .

gr:Maintain rdfs:label "Maintain (business function)"@en .

gr:BusinessFunction rdfs:label "Business function"@en .

gr:hasOpeningHoursSpecification rdfs:label "has opening hours specification (0..*)"@en .

gr:validThrough rdfs:label "valid through (0..1)"@en .

gr:License rdfs:label "License"@en .

gr:AmericanExpress rdfs:label "American Express (payment method)"@en .

gr:PaymentMethodCreditCard rdfs:label "Payment method credit card"@en .

gr:appliesToPaymentMethod rdfs:label "applies to payment method (1..*)"@en .

gr:PaymentChargeSpecification rdfs:label "Payment charge specification"@en .

gr:isConsumableFor rdfs:label "is consumable for (0..*)"@en .

gr:hasValueFloat rdfs:label "has value float (0..1)"@en .

gr:hasMaxValueFloat rdfs:label "has max value float (1..1)"@en .

gr:hasMaxValue rdfs:label "has max value (0..1)"@en .

gr:hasMinValueFloat rdfs:label "has min value float (1..1)"@en .

gr:hasMinValue rdfs:label "has min value (0..1)"@en .

gr:closes rdfs:label "closes (1..1)"@en .

gr:PaySwarm rdfs:label "PaySwarm (payment method)"@en .

gr:advanceBookingRequirement rdfs:label "advance booking requirement (0..1)"@en .

gr:eligibleTransactionVolume rdfs:label "eligible transaction volume (0..1)"@en .

gr:durationOfWarrantyInMonths rdfs:label "duration of warranty in months (0..1)"@en .

gr:WarrantyPromise rdfs:label "Warranty promise"@en .

gr:hasGlobalLocationNumber rdfs:label "has Global Location Number (0..1)"@en .

gr:isVariantOf rdfs:label "is variant of (0..1)"@en .

gr:ProductOrServiceModel rdfs:label "Product or service model"@en .

gr:hasGTIN-8 rdfs:label "has GTIN-8 (0..*)"@en .

gr:PartsAndLabor-PickUp rdfs:label "Parts and labor / pick up (warranty scope)"@en .

gr:WarrantyScope rdfs:label "Warranty scope"@en .

gr:JCB rdfs:label "JCB (payment method)"@en .

gr:depth rdfs:label "depth (0..1)"@en .

gr:QuantitativeValue rdfs:label "Quantitative value"@en .

gr:quantitativeProductOrServiceProperty rdfs:label "quantitative product or service property (0..*)"@en .

gr:hasValueInteger rdfs:label "has value integer (0..1)"@en .

gr:hasMinValueInteger rdfs:label "has min value integer (1..1)"@en .

gr:hasMaxValueInteger rdfs:label "has max value integer (1..1)"@en .

gr:hasManufacturer rdfs:label "has manufacturer (0..1)"@en .

gr:description rdfs:label "description (0..1)"@en .

gr:Brand rdfs:label "Brand"@en .

gr:DayOfWeek rdfs:label "Day of week"@en .

gr:DeliveryChargeSpecification rdfs:label "Delivery charge specification"@en .

gr:QualitativeValue rdfs:label "Qualitative value"@en .

gr:UnitPriceSpecification rdfs:label "Unit price specification"@en .

gr:Cash rdfs:label "Cash (payment method)"@en .

gr:DinersClub rdfs:label "Diners Club (payment method)"@en .

gr:Dispose rdfs:label "Dispose (business function)"@en .

gr:billingIncrement rdfs:label "billing increment (0..1)"@en .

gr:isListPrice rdfs:label "is list price (DEPRECATED)"@en .

gr:color rdfs:label "color (0..1)"@en .

gr:datatypeProductOrServiceProperty rdfs:label "datatype product or service property (0..*)"@en .

gr:isAccessoryOrSparePartFor rdfs:label "is accessory or spare part for (0..*)"@en .

gr:hasDUNS rdfs:label "has DUNS (0..1)"@en .

gr:typeOfGood rdfs:label "type of good (1..1)"@en .

gr:deliveryLeadTime rdfs:label "delivery lead time (0..1)"@en .

gr:hasStockKeepingUnit rdfs:label "has Stock Keeping Unit (0..*)"@en .

gr:qualitativeProductOrServiceProperty rdfs:label "qualitative product or service property (0..*)"@en .

gr:availableDeliveryMethods rdfs:label "available delivery methods (0..*)"@en .

gr:Repair rdfs:label "Repair (business function)"@en .

gr:GoogleCheckout rdfs:label "Google Checkout (payment method)"@en .

gr:includes rdfs:label "includes (0..1)"@en .

gr:Business rdfs:label "Business (business entity type)"@en .

gr:Sell rdfs:label "Sell (business function)"@en .

gr:hasValue rdfs:label "has value (0..1)"@en .

gr:hasBrand rdfs:label "has brand (0..*)"@en .

gr:ByBankTransferInAdvance rdfs:label "By bank transfer in advance (payment method)"@en .

gr:hasOpeningHoursDayOfWeek rdfs:label "has opening hours day of week (1..*)"@en .

gr:priceType rdfs:label "price type (0..1)"@en .

gr:DeliveryModeOwnFleet rdfs:label "Delivery mode own fleet (delivery method)"@en .

gr:eligibleRegions rdfs:label "eligible regions (0..*)"@en .

gr:VISA rdfs:label "VISA (payment method)"@en .

gr:valueReference rdfs:label "value reference (0..*)"@en .

gr:validFrom rdfs:label "valid from (0..1)"@en .

gr:DeliveryModeDirectDownload rdfs:label "Delivery mode direct download (delivery method)"@en .

gr:UPS rdfs:label "UPS (delivery method)"@en .

gr:ConstructionInstallation rdfs:label "Construction / installation (business function)"@en .

gr:CheckInAdvance rdfs:label "Check in advance (payment method)"@en .

gr:name rdfs:label "name (0..1)"@en .

gr:hasWarrantyPromise rdfs:label "has warranty promise (0..*)"@en .

gr:hasGTIN-14 rdfs:label "has GTIN-14 (0..*)"@en .

gr:LeaseOut rdfs:label "Lease Out (business function)"@en .

gr:hasCurrencyValue rdfs:label "has currency value (0..1)"@en .

gr:hasMinCurrencyValue rdfs:label "has min currency value (1..1)"@en .

gr:hasMaxCurrencyValue rdfs:label "has max currency value (1..1)"@en .

gr:hasCurrency rdfs:label "has currency (1..1)"@en .

gr:Buy rdfs:label "Buy (business function, DEPRECATED)"@en .

gr:hasMakeAndModel rdfs:label "has make and model (0..1)"@en .

gr:PartsAndLabor-BringIn rdfs:label "Parts and labor / bring-in (warranty scope)"@en .

gr:Enduser rdfs:label "Enduser (business entity type)"@en .

gr:relatedWebService rdfs:label "related Web Service (0..*)"@en .

gr:PublicHolidays rdfs:label "Public holidays (day of week)"@en .

gr:displayPosition rdfs:label "display position (0..1)"@en .

gr:valueAddedTaxIncluded rdfs:label "value added tax included (0..1)"@en .

gr:acceptedPaymentMethods rdfs:label "accepted payment methods (0..*)"@en .

gr:hasBusinessFunction rdfs:label "has business function (1..*)"@en .

gr:hasWarrantyScope rdfs:label "has warranty scope (0..1)"@en .

gr:weight rdfs:label "weight (0..1)"@en .

gr:includesObject rdfs:label "includes object (0..*)"@en .

gr:hasEAN_UCC-13 rdfs:label "has EAN/UCC-13 (0..*)"@en .

gr:N-Ary-Relations rdfs:label "N-ary relations (DEPRECATED)"@en .

gr:equal rdfs:label "equal (0..*)"@en .

gr:Labor-BringIn rdfs:label "Labor / bring-in (warranty scope)"@en .

gr:height rdfs:label "height (0..1)"@en .

gr:width rdfs:label "width (0..1)"@en .

gr:COD rdfs:label "COD (payment method)"@en .

gr:hasEligibleQuantity rdfs:label "has eligible quantity (0..1)"@en .

gr:DeliveryModeFreight rdfs:label "Delivery mode freight (delivery method)"@en .

gr:eligibleDuration rdfs:label "eligible duration (0..1)"@en .

gr:PayPal rdfs:label "PayPal (payment method)"@en .

gr:nonEqual rdfs:label "non equal (0..*)"@en .

gr:condition rdfs:label "condition (0..1)"@en .

gr:PublicInstitution rdfs:label "Public institution (business entity type)"@en .

gr:DeliveryModePickUp rdfs:label "Delivery mode pick up (delivery method)"@en .

gr:Discover rdfs:label "Discover (payment method)"@en .

gr:DirectDebit rdfs:label "Direct debit (payment method)"@en .

gr:ProvideService rdfs:label "Provide service (business function)"@en .

gr:appliesToDeliveryMethod rdfs:label "applies to delivery method (0..*)"@en .

gr:owns rdfs:label "owns (0..*)"@en .

gr:MasterCard rdfs:label "MasterCard (payment method)"@en .

gr:hasUnitOfMeasurement rdfs:label "has unit of measurement (1..1)"@en .

gr:offers rdfs:label "offers (0..*)"@en .

gr:addOn rdfs:label "add-on (0..*)"@en .

gr:Wednesday rdfs:label "Wednesday (day of week)"@en .

gr:hasNext rdfs:label "has next (0..1)"@en .

gr:Thursday rdfs:label "Thursday (day of week)"@en .

gr:Friday rdfs:label "Friday (day of week)"@en .

gr:hasPrevious rdfs:label "has previous (0..1)"@en .

gr:Tuesday rdfs:label "Tuesday (day of week)"@en .

gr:Monday rdfs:label "Monday (day of week)"@en .

gr:lesser rdfs:label "lesser (0..*)"@en .

gr:greater rdfs:label "greater (0..*)"@en .

gr:LocationOfSalesOrServiceProvisioning rdfs:label "Location of sales or service provisioning (DEPRECATED)"@en .

gr:ProductOrServicesSomeInstancesPlaceholder rdfs:label "Product or services some instances placeholder (DEPRECATED)"@en .

gr:predecessorOf rdfs:label "predecessor of (0..*)"@en .

gr:successorOf rdfs:label "successor of (0..*)"@en .

gr:Sunday rdfs:label "Sunday (day of week)"@en .

gr:Saturday rdfs:label "Saturday (day of week)"@en .

gr:ActualProductOrServiceInstance rdfs:label "Actual product or service instance (DEPRECATED)"@en .

gr:greaterOrEqual rdfs:label "greater or equal (0..*)"@en .

gr:lesserOrEqual rdfs:label "lesser or equal (0..*)"@en .

pc:Contract rdfs:isDefinedBy <http://purl.org/procurement/public-contracts> .

pc:FrameworkAgreement rdfs:isDefinedBy <http://purl.org/procurement/public-contracts> .

pc:Tender rdfs:isDefinedBy <http://purl.org/procurement/public-contracts> .

gr:Offering rdfs:isDefinedBy <http://purl.org/goodrelations/v1> .

pc:AwardCriteriaCombination rdfs:isDefinedBy <http://purl.org/procurement/public-contracts> .

pc:CriterionWeighting rdfs:isDefinedBy <http://purl.org/procurement/public-contracts> .

pc:TendersOpening rdfs:isDefinedBy <http://purl.org/procurement/public-contracts> .

pc:awardDate rdfs:isDefinedBy <http://purl.org/procurement/public-contracts> .

pc:contact rdfs:isDefinedBy <http://purl.org/procurement/public-contracts> .

pc:kind rdfs:isDefinedBy <http://purl.org/procurement/public-contracts> .

pc:procedureType rdfs:isDefinedBy <http://purl.org/procurement/public-contracts> .

pc:contractingAuthority rdfs:isDefinedBy <http://purl.org/procurement/public-contracts> .

gr:BusinessEntity rdfs:isDefinedBy <http://purl.org/goodrelations/v1> .

pc:item rdfs:isDefinedBy <http://purl.org/procurement/public-contracts> .

pc:mainObject rdfs:isDefinedBy <http://purl.org/procurement/public-contracts> .

pc:additionalObject rdfs:isDefinedBy <http://purl.org/procurement/public-contracts> .

pc:location rdfs:isDefinedBy <http://purl.org/procurement/public-contracts> .

pc:contractPrice rdfs:isDefinedBy <http://purl.org/procurement/public-contracts> .

gr:PriceSpecification rdfs:isDefinedBy <http://purl.org/goodrelations/v1> .

pc:documentationPrice rdfs:isDefinedBy <http://purl.org/procurement/public-contracts> .

pc:estimatedPrice rdfs:isDefinedBy <http://purl.org/procurement/public-contracts> .

pc:tenderDeadline rdfs:isDefinedBy <http://purl.org/procurement/public-contracts> .

pc:documentationRequestDeadline rdfs:isDefinedBy <http://purl.org/procurement/public-contracts> .

pc:duration rdfs:isDefinedBy <http://purl.org/procurement/public-contracts> .

pc:tenderMaintenanceDuration rdfs:isDefinedBy <http://purl.org/procurement/public-contracts> .

pc:startDate rdfs:isDefinedBy <http://purl.org/procurement/public-contracts> .

pc:estimatedEndDate rdfs:isDefinedBy <http://purl.org/procurement/public-contracts> .

pc:actualEndDate rdfs:isDefinedBy <http://purl.org/procurement/public-contracts> .

pc:awardCriteriaCombination rdfs:isDefinedBy <http://purl.org/procurement/public-contracts> .

pc:lot rdfs:isDefinedBy <http://purl.org/procurement/public-contracts> .

pc:frameworkAgreement rdfs:isDefinedBy <http://purl.org/procurement/public-contracts> .

pc:numberOfTenders rdfs:isDefinedBy <http://purl.org/procurement/public-contracts> .

pc:tender rdfs:isDefinedBy <http://purl.org/procurement/public-contracts> .

pc:awardedTender rdfs:isDefinedBy <http://purl.org/procurement/public-contracts> .

pc:subsidy rdfs:isDefinedBy <http://purl.org/procurement/public-contracts> .

pc:agreedPrice rdfs:isDefinedBy <http://purl.org/procurement/public-contracts> .

pc:actualPrice rdfs:isDefinedBy <http://purl.org/procurement/public-contracts> .

pc:attachment rdfs:isDefinedBy <http://purl.org/procurement/public-contracts> .

pc:specification rdfs:isDefinedBy <http://purl.org/procurement/public-contracts> .

pc:agreement rdfs:isDefinedBy <http://purl.org/procurement/public-contracts> .

pc:awardCriterion rdfs:isDefinedBy <http://purl.org/procurement/public-contracts> .

pc:expectedNumberOfOperators rdfs:isDefinedBy <http://purl.org/procurement/public-contracts> .

gr:QuantitativeValueInteger rdfs:isDefinedBy <http://purl.org/goodrelations/v1> .

pc:profile rdfs:isDefinedBy <http://purl.org/procurement/public-contracts> .

pc:authorityKind rdfs:isDefinedBy <http://purl.org/procurement/public-contracts> .

pc:mainActivity rdfs:isDefinedBy <http://purl.org/procurement/public-contracts> .

pc:offeredPrice rdfs:isDefinedBy <http://purl.org/procurement/public-contracts> .

gr:hasPriceSpecification rdfs:isDefinedBy <http://purl.org/goodrelations/v1> .

pc:bidder rdfs:isDefinedBy <http://purl.org/procurement/public-contracts> .

pc:contract rdfs:isDefinedBy <http://purl.org/procurement/public-contracts> .

pc:weightedCriterion rdfs:isDefinedBy <http://purl.org/procurement/public-contracts> .

pc:criterionWeight rdfs:isDefinedBy <http://purl.org/procurement/public-contracts> .

gr:availabilityStarts rdfs:isDefinedBy <http://purl.org/goodrelations/v1> .

gr:availableAtOrFrom rdfs:isDefinedBy <http://purl.org/goodrelations/v1> .

gr:Location rdfs:isDefinedBy <http://purl.org/goodrelations/v1> .

gr:taxID rdfs:isDefinedBy <http://purl.org/goodrelations/v1> .

gr:seeks rdfs:isDefinedBy <http://purl.org/goodrelations/v1> .

gr:Reseller rdfs:isDefinedBy <http://purl.org/goodrelations/v1> .

gr:BusinessEntityType rdfs:isDefinedBy <http://purl.org/goodrelations/v1> .

gr:amountOfThisGood rdfs:isDefinedBy <http://purl.org/goodrelations/v1> .

gr:TypeAndQuantityNode rdfs:isDefinedBy <http://purl.org/goodrelations/v1> .

gr:serialNumber rdfs:isDefinedBy <http://purl.org/goodrelations/v1> .

gr:Individual rdfs:isDefinedBy <http://purl.org/goodrelations/v1> .

gr:hasISICv4 rdfs:isDefinedBy <http://purl.org/goodrelations/v1> .

gr:opens rdfs:isDefinedBy <http://purl.org/goodrelations/v1> .

gr:OpeningHoursSpecification rdfs:isDefinedBy <http://purl.org/goodrelations/v1> .

gr:hasNAICS rdfs:isDefinedBy <http://purl.org/goodrelations/v1> .

gr:legalName rdfs:isDefinedBy <http://purl.org/goodrelations/v1> .

gr:FederalExpress rdfs:isDefinedBy <http://purl.org/goodrelations/v1> .

gr:DeliveryModeParcelService rdfs:isDefinedBy <http://purl.org/goodrelations/v1> .

gr:hasMPN rdfs:isDefinedBy <http://purl.org/goodrelations/v1> .

gr:ProductOrService rdfs:isDefinedBy <http://purl.org/goodrelations/v1> .

gr:vatID rdfs:isDefinedBy <http://purl.org/goodrelations/v1> .

gr:DHL rdfs:isDefinedBy <http://purl.org/goodrelations/v1> .

gr:DeliveryModeMail rdfs:isDefinedBy <http://purl.org/goodrelations/v1> .

gr:DeliveryMethod rdfs:isDefinedBy <http://purl.org/goodrelations/v1> .

gr:category rdfs:isDefinedBy <http://purl.org/goodrelations/v1> .

gr:hasPOS rdfs:isDefinedBy <http://purl.org/goodrelations/v1> .

gr:availabilityEnds rdfs:isDefinedBy <http://purl.org/goodrelations/v1> .

gr:eligibleCustomerTypes rdfs:isDefinedBy <http://purl.org/goodrelations/v1> .

gr:ByInvoice rdfs:isDefinedBy <http://purl.org/goodrelations/v1> .

gr:PaymentMethod rdfs:isDefinedBy <http://purl.org/goodrelations/v1> .

gr:hasInventoryLevel rdfs:isDefinedBy <http://purl.org/goodrelations/v1> .

gr:QuantitativeValueFloat rdfs:isDefinedBy <http://purl.org/goodrelations/v1> .

gr:SomeItems rdfs:isDefinedBy <http://purl.org/goodrelations/v1> .

gr:isSimilarTo rdfs:isDefinedBy <http://purl.org/goodrelations/v1> .

gr:Maintain rdfs:isDefinedBy <http://purl.org/goodrelations/v1> .

gr:BusinessFunction rdfs:isDefinedBy <http://purl.org/goodrelations/v1> .

gr:hasOpeningHoursSpecification rdfs:isDefinedBy <http://purl.org/goodrelations/v1> .

gr:validThrough rdfs:isDefinedBy <http://purl.org/goodrelations/v1> .

gr:License rdfs:isDefinedBy <http://purl.org/goodrelations/v1> .

gr:AmericanExpress rdfs:isDefinedBy <http://purl.org/goodrelations/v1> .

gr:PaymentMethodCreditCard rdfs:isDefinedBy <http://purl.org/goodrelations/v1> .

gr:appliesToPaymentMethod rdfs:isDefinedBy <http://purl.org/goodrelations/v1> .

gr:PaymentChargeSpecification rdfs:isDefinedBy <http://purl.org/goodrelations/v1> .

gr:isConsumableFor rdfs:isDefinedBy <http://purl.org/goodrelations/v1> .

gr:hasValueFloat rdfs:isDefinedBy <http://purl.org/goodrelations/v1> .

gr:hasMaxValueFloat rdfs:isDefinedBy <http://purl.org/goodrelations/v1> .

gr:hasMaxValue rdfs:isDefinedBy <http://purl.org/goodrelations/v1> .

gr:hasMinValueFloat rdfs:isDefinedBy <http://purl.org/goodrelations/v1> .

gr:hasMinValue rdfs:isDefinedBy <http://purl.org/goodrelations/v1> .

gr:closes rdfs:isDefinedBy <http://purl.org/goodrelations/v1> .

gr:PaySwarm rdfs:isDefinedBy <http://purl.org/goodrelations/v1> .

gr:advanceBookingRequirement rdfs:isDefinedBy <http://purl.org/goodrelations/v1> .

gr:eligibleTransactionVolume rdfs:isDefinedBy <http://purl.org/goodrelations/v1> .

gr:durationOfWarrantyInMonths rdfs:isDefinedBy <http://purl.org/goodrelations/v1> .

gr:WarrantyPromise rdfs:isDefinedBy <http://purl.org/goodrelations/v1> .

gr:hasGlobalLocationNumber rdfs:isDefinedBy <http://purl.org/goodrelations/v1> .

gr:isVariantOf rdfs:isDefinedBy <http://purl.org/goodrelations/v1> .

gr:ProductOrServiceModel rdfs:isDefinedBy <http://purl.org/goodrelations/v1> .

gr:hasGTIN-8 rdfs:isDefinedBy <http://purl.org/goodrelations/v1> .

gr:PartsAndLabor-PickUp rdfs:isDefinedBy <http://purl.org/goodrelations/v1> .

gr:WarrantyScope rdfs:isDefinedBy <http://purl.org/goodrelations/v1> .

gr:JCB rdfs:isDefinedBy <http://purl.org/goodrelations/v1> .

gr:depth rdfs:isDefinedBy <http://purl.org/goodrelations/v1> .

gr:QuantitativeValue rdfs:isDefinedBy <http://purl.org/goodrelations/v1> .

gr:quantitativeProductOrServiceProperty rdfs:isDefinedBy <http://purl.org/goodrelations/v1> .

gr:hasValueInteger rdfs:isDefinedBy <http://purl.org/goodrelations/v1> .

gr:hasMinValueInteger rdfs:isDefinedBy <http://purl.org/goodrelations/v1> .

gr:hasMaxValueInteger rdfs:isDefinedBy <http://purl.org/goodrelations/v1> .

gr:hasManufacturer rdfs:isDefinedBy <http://purl.org/goodrelations/v1> .

gr:description rdfs:isDefinedBy <http://purl.org/goodrelations/v1> .

gr:Brand rdfs:isDefinedBy <http://purl.org/goodrelations/v1> .

gr:DayOfWeek rdfs:isDefinedBy <http://purl.org/goodrelations/v1> .

gr:DeliveryChargeSpecification rdfs:isDefinedBy <http://purl.org/goodrelations/v1> .

gr:QualitativeValue rdfs:isDefinedBy <http://purl.org/goodrelations/v1> .

gr:UnitPriceSpecification rdfs:isDefinedBy <http://purl.org/goodrelations/v1> .

gr:Cash rdfs:isDefinedBy <http://purl.org/goodrelations/v1> .

gr:DinersClub rdfs:isDefinedBy <http://purl.org/goodrelations/v1> .

gr:Dispose rdfs:isDefinedBy <http://purl.org/goodrelations/v1> .

gr:billingIncrement rdfs:isDefinedBy <http://purl.org/goodrelations/v1> .

gr:isListPrice rdfs:isDefinedBy <http://purl.org/goodrelations/v1> .

gr:color rdfs:isDefinedBy <http://purl.org/goodrelations/v1> .

gr:datatypeProductOrServiceProperty rdfs:isDefinedBy <http://purl.org/goodrelations/v1> .

gr:isAccessoryOrSparePartFor rdfs:isDefinedBy <http://purl.org/goodrelations/v1> .

gr:hasDUNS rdfs:isDefinedBy <http://purl.org/goodrelations/v1> .

gr:typeOfGood rdfs:isDefinedBy <http://purl.org/goodrelations/v1> .

gr:deliveryLeadTime rdfs:isDefinedBy <http://purl.org/goodrelations/v1> .

gr:hasStockKeepingUnit rdfs:isDefinedBy <http://purl.org/goodrelations/v1> .

gr:qualitativeProductOrServiceProperty rdfs:isDefinedBy <http://purl.org/goodrelations/v1> .

gr:availableDeliveryMethods rdfs:isDefinedBy <http://purl.org/goodrelations/v1> .

gr:Repair rdfs:isDefinedBy <http://purl.org/goodrelations/v1> .

gr:GoogleCheckout rdfs:isDefinedBy <http://purl.org/goodrelations/v1> .

gr:includes rdfs:isDefinedBy <http://purl.org/goodrelations/v1> .

gr:Business rdfs:isDefinedBy <http://purl.org/goodrelations/v1> .

gr:Sell rdfs:isDefinedBy <http://purl.org/goodrelations/v1> .

gr:hasValue rdfs:isDefinedBy <http://purl.org/goodrelations/v1> .

gr:hasBrand rdfs:isDefinedBy <http://purl.org/goodrelations/v1> .

gr:ByBankTransferInAdvance rdfs:isDefinedBy <http://purl.org/goodrelations/v1> .

gr:hasOpeningHoursDayOfWeek rdfs:isDefinedBy <http://purl.org/goodrelations/v1> .

gr:priceType rdfs:isDefinedBy <http://purl.org/goodrelations/v1> .

gr:DeliveryModeOwnFleet rdfs:isDefinedBy <http://purl.org/goodrelations/v1> .

gr:eligibleRegions rdfs:isDefinedBy <http://purl.org/goodrelations/v1> .

gr:VISA rdfs:isDefinedBy <http://purl.org/goodrelations/v1> .

gr:valueReference rdfs:isDefinedBy <http://purl.org/goodrelations/v1> .

gr:validFrom rdfs:isDefinedBy <http://purl.org/goodrelations/v1> .

gr:DeliveryModeDirectDownload rdfs:isDefinedBy <http://purl.org/goodrelations/v1> .

gr:UPS rdfs:isDefinedBy <http://purl.org/goodrelations/v1> .

gr:ConstructionInstallation rdfs:isDefinedBy <http://purl.org/goodrelations/v1> .

gr:CheckInAdvance rdfs:isDefinedBy <http://purl.org/goodrelations/v1> .

gr:name rdfs:isDefinedBy <http://purl.org/goodrelations/v1> .

gr:hasWarrantyPromise rdfs:isDefinedBy <http://purl.org/goodrelations/v1> .

gr:hasGTIN-14 rdfs:isDefinedBy <http://purl.org/goodrelations/v1> .

gr:LeaseOut rdfs:isDefinedBy <http://purl.org/goodrelations/v1> .

gr:hasCurrencyValue rdfs:isDefinedBy <http://purl.org/goodrelations/v1> .

gr:hasMinCurrencyValue rdfs:isDefinedBy <http://purl.org/goodrelations/v1> .

gr:hasMaxCurrencyValue rdfs:isDefinedBy <http://purl.org/goodrelations/v1> .

gr:hasCurrency rdfs:isDefinedBy <http://purl.org/goodrelations/v1> .

gr:Buy rdfs:isDefinedBy <http://purl.org/goodrelations/v1> .

gr:hasMakeAndModel rdfs:isDefinedBy <http://purl.org/goodrelations/v1> .

gr:PartsAndLabor-BringIn rdfs:isDefinedBy <http://purl.org/goodrelations/v1> .

gr:Enduser rdfs:isDefinedBy <http://purl.org/goodrelations/v1> .

gr:relatedWebService rdfs:isDefinedBy <http://purl.org/goodrelations/v1> .

gr:PublicHolidays rdfs:isDefinedBy <http://purl.org/goodrelations/v1> .

gr:displayPosition rdfs:isDefinedBy <http://purl.org/goodrelations/v1> .

gr:valueAddedTaxIncluded rdfs:isDefinedBy <http://purl.org/goodrelations/v1> .

gr:acceptedPaymentMethods rdfs:isDefinedBy <http://purl.org/goodrelations/v1> .

gr:hasBusinessFunction rdfs:isDefinedBy <http://purl.org/goodrelations/v1> .

gr:hasWarrantyScope rdfs:isDefinedBy <http://purl.org/goodrelations/v1> .

gr:weight rdfs:isDefinedBy <http://purl.org/goodrelations/v1> .

gr:includesObject rdfs:isDefinedBy <http://purl.org/goodrelations/v1> .

gr:hasEAN_UCC-13 rdfs:isDefinedBy <http://purl.org/goodrelations/v1> .

gr:N-Ary-Relations rdfs:isDefinedBy <http://purl.org/goodrelations/v1> .

gr:equal rdfs:isDefinedBy <http://purl.org/goodrelations/v1> .

gr:Labor-BringIn rdfs:isDefinedBy <http://purl.org/goodrelations/v1> .

gr:height rdfs:isDefinedBy <http://purl.org/goodrelations/v1> .

gr:width rdfs:isDefinedBy <http://purl.org/goodrelations/v1> .

gr:COD rdfs:isDefinedBy <http://purl.org/goodrelations/v1> .

gr:hasEligibleQuantity rdfs:isDefinedBy <http://purl.org/goodrelations/v1> .

gr:DeliveryModeFreight rdfs:isDefinedBy <http://purl.org/goodrelations/v1> .

gr:eligibleDuration rdfs:isDefinedBy <http://purl.org/goodrelations/v1> .

gr:PayPal rdfs:isDefinedBy <http://purl.org/goodrelations/v1> .

gr:nonEqual rdfs:isDefinedBy <http://purl.org/goodrelations/v1> .

gr:condition rdfs:isDefinedBy <http://purl.org/goodrelations/v1> .

gr:PublicInstitution rdfs:isDefinedBy <http://purl.org/goodrelations/v1> .

gr:DeliveryModePickUp rdfs:isDefinedBy <http://purl.org/goodrelations/v1> .

gr:Discover rdfs:isDefinedBy <http://purl.org/goodrelations/v1> .

gr:DirectDebit rdfs:isDefinedBy <http://purl.org/goodrelations/v1> .

gr:ProvideService rdfs:isDefinedBy <http://purl.org/goodrelations/v1> .

gr:appliesToDeliveryMethod rdfs:isDefinedBy <http://purl.org/goodrelations/v1> .

gr:owns rdfs:isDefinedBy <http://purl.org/goodrelations/v1> .

gr:MasterCard rdfs:isDefinedBy <http://purl.org/goodrelations/v1> .

gr:hasUnitOfMeasurement rdfs:isDefinedBy <http://purl.org/goodrelations/v1> .

gr:offers rdfs:isDefinedBy <http://purl.org/goodrelations/v1> .

gr:addOn rdfs:isDefinedBy <http://purl.org/goodrelations/v1> .

gr:Wednesday rdfs:isDefinedBy <http://purl.org/goodrelations/v1> .

gr:hasNext rdfs:isDefinedBy <http://purl.org/goodrelations/v1> .

gr:Thursday rdfs:isDefinedBy <http://purl.org/goodrelations/v1> .

gr:Friday rdfs:isDefinedBy <http://purl.org/goodrelations/v1> .

gr:hasPrevious rdfs:isDefinedBy <http://purl.org/goodrelations/v1> .

gr:Tuesday rdfs:isDefinedBy <http://purl.org/goodrelations/v1> .

gr:Monday rdfs:isDefinedBy <http://purl.org/goodrelations/v1> .

gr:lesser rdfs:isDefinedBy <http://purl.org/goodrelations/v1> .

gr:greater rdfs:isDefinedBy <http://purl.org/goodrelations/v1> .

gr:LocationOfSalesOrServiceProvisioning rdfs:isDefinedBy <http://purl.org/goodrelations/v1> .

gr:ProductOrServicesSomeInstancesPlaceholder rdfs:isDefinedBy <http://purl.org/goodrelations/v1> .

gr:predecessorOf rdfs:isDefinedBy <http://purl.org/goodrelations/v1> .

gr:successorOf rdfs:isDefinedBy <http://purl.org/goodrelations/v1> .

gr:Sunday rdfs:isDefinedBy <http://purl.org/goodrelations/v1> .

gr:Saturday rdfs:isDefinedBy <http://purl.org/goodrelations/v1> .

gr:ActualProductOrServiceInstance rdfs:isDefinedBy <http://purl.org/goodrelations/v1> .

gr:greaterOrEqual rdfs:isDefinedBy <http://purl.org/goodrelations/v1> .

gr:lesserOrEqual rdfs:isDefinedBy <http://purl.org/goodrelations/v1> .

<http://purl.org/procurement/public-contracts> rdfs:seeAlso <https://github.com/opendatacz/public-contracts-ontology>,
    <http://prefix.cc/pc>;
  dcterms:title "Public Contracts Ontology"@en, "Ontologie pro veřejné zakázky"@cs;
  dcterms:description "Ontologie pro veřejné zakázky poskytuje vyjadřovací prostředky pro popis zakázek zadávaných institucemi veřejné správy."@cs,
    "Public Contracts Ontology offers a means of expression for describing public contracts in the public sector."@en;
  dcterms:modified "2012-10-10"^^xsd:date;
  vann:preferredNamespaceUri "http://purl.org/procurement/public-contracts#";
  vann:preferredNamespacePrefix "pc";
  dcterms:creator <http://purl.org/klimek#me>, <http://purl.org/knap#me>, <http://mynarz.net/#jindrich>,
    <http://www.ksi.mff.cuni.cz/~necasky>, <http://www.facebook.com/nohis>, <http://keg.vse.cz/resource/person/josef-petrak>,
    <http://keg.vse.cz/resource/person/vojtech-svatek>;
  dcterms:rights <http://creativecommons.org/licenses/by/3.0/cz/> .

<http://purl.org/klimek#me> foaf:name "Jakub Klímek" .

<http://purl.org/knap#me> foaf:name "Tomáš Knap" .

<http://www.ksi.mff.cuni.cz/~necasky> foaf:name "Martin Nečaský" .

<http://www.facebook.com/nohis> foaf:name "Pavel Nohejl" .

<http://keg.vse.cz/resource/person/josef-petrak> foaf:name "Josef Petrák" .

<http://keg.vse.cz/resource/person/vojtech-svatek> foaf:name "Vojtěch Svátek" .

<http://keg.vse.cz/resource/person/jindrich-mynarz> foaf:name "Jindřich Mynarz" .

<http://purl.org/klimek#me> foaf:mbox <mailto:klimek.mff@gmail.com> .

<http://purl.org/knap#me> foaf:mbox <mailto:toknap@gmail.com> .

<http://www.ksi.mff.cuni.cz/~necasky> foaf:mbox <mailto:martinnec@gmail.com> .

<http://www.facebook.com/nohis> foaf:mbox <mailto:nohejl.pavel@gmail.com> .

<http://keg.vse.cz/resource/person/josef-petrak> foaf:mbox <mailto:me@jspetrak.name> .

<http://keg.vse.cz/resource/person/vojtech-svatek> foaf:mbox <mailto:svatek@vse.cz> .

<http://keg.vse.cz/resource/person/jindrich-mynarz> foaf:mbox <mailto:mynarzjindrich@gmail.com> .

dcterms:title vann:usageNote "Use for labelling states of public contracts (instances of pc:Contract). The domain is pc:Contract."@en .

dcterms:description vann:usageNote "Use for attaching plain text description of public contracts (instances of pc:Contract). The domain is pc:Contract."@en .

adms:identifier vann:usageNote "Use for attaching identifiers (instances of adms:Identifier) to contracting authorities and bidders (instances of gr:BusinessEntity). The property should be used for official numbers assigned to public contracts in national public procurement systems, reference numbers of public contracts assigned by their contracting authorities, notice number in EU TED, etc. The domain is a union of gr:BusinessEntity and pc:Contract."@en .

dcterms:date vann:usageNote "Use for date and time, when tenders are opened. The domain is pc:TendersOpening. Cardinality 0..1"@en,
    "Používejte pro datum a čas otevření nabídek. Definičním oborem je pc:TendersOpening. Kardinalita 0..1"@cs .

schema:location vann:usageNote "Use for location, where tenders are opened. The domain is pc:TendersOpening. Cardinality 0..1"@en,
    "Místo, kde dojde k otevření obálek s nabídkami pro veřejnou zakázku. Definičním oborem je pc:TendersOpening. Kardinalita 0..1"@cs .

_:node155 rdf:rest _:node156 .

_:node156 rdf:rest rdf:nil .

_:node158 rdf:rest _:node159 .

_:node159 rdf:rest _:node160 .

_:node160 rdf:rest _:node161 .

_:node161 rdf:rest rdf:nil .

_:node163 rdf:rest _:node164 .

_:node164 rdf:rest rdf:nil .

_:node167 rdf:rest _:node168 .

_:node168 rdf:rest rdf:nil .

_:node170 rdf:rest _:node171 .

_:node171 rdf:rest _:node172 .

_:node172 rdf:rest _:node173 .

_:node173 rdf:rest rdf:nil .

_:node175 rdf:rest _:node176 .

_:node176 rdf:rest _:node177 .

_:node177 rdf:rest _:node178 .

_:node178 rdf:rest rdf:nil .

_:node180 rdf:rest _:node181 .

_:node181 rdf:rest rdf:nil .

_:node183 rdf:rest _:node184 .

_:node184 rdf:rest rdf:nil .

_:node186 rdf:rest _:node187 .

_:node187 rdf:rest _:node188 .

_:node188 rdf:rest _:node189 .

_:node189 rdf:rest _:node190 .

_:node190 rdf:rest rdf:nil .

_:node192 rdf:rest _:node193 .

_:node193 rdf:rest _:node194 .

_:node194 rdf:rest _:node195 .

_:node195 rdf:rest _:node196 .

_:node196 rdf:rest _:node197 .

_:node197 rdf:rest _:node198 .

_:node198 rdf:rest _:node199 .

_:node199 rdf:rest _:node200 .

_:node200 rdf:rest _:node201 .

_:node201 rdf:rest _:node202 .

_:node202 rdf:rest _:node203 .

_:node203 rdf:rest _:node204 .

_:node204 rdf:rest _:node205 .

_:node205 rdf:rest _:node206 .

_:node206 rdf:rest _:node207 .

_:node207 rdf:rest _:node208 .

_:node208 rdf:rest _:node209 .

_:node209 rdf:rest _:node210 .

_:node210 rdf:rest _:node211 .

_:node211 rdf:rest _:node212 .

_:node212 rdf:rest _:node213 .

_:node213 rdf:rest _:node214 .

_:node214 rdf:rest _:node215 .

_:node215 rdf:rest _:node216 .

_:node216 rdf:rest _:node217 .

_:node217 rdf:rest _:node218 .

_:node218 rdf:rest _:node219 .

_:node219 rdf:rest rdf:nil .

_:node221 rdf:rest _:node222 .

_:node222 rdf:rest rdf:nil .

_:node224 rdf:rest _:node225 .

_:node225 rdf:rest _:node226 .

_:node226 rdf:rest rdf:nil .

_:node228 rdf:rest _:node229 .

_:node229 rdf:rest _:node230 .

_:node230 rdf:rest rdf:nil .

_:node232 rdf:rest _:node233 .

_:node233 rdf:rest rdf:nil .

_:node235 rdf:rest _:node236 .

_:node236 rdf:rest _:node237 .

_:node237 rdf:rest rdf:nil .

_:node239 rdf:rest _:node240 .

_:node240 rdf:rest rdf:nil .

<http://purl.org/goodrelations/v1> dc:title "The GoodRelations Vocabulary for Semantic Web-based E-Commerce"@en;
  dc:subject "E-Commerce, E-Business, GoodRelations, Microdata, Ontology, Semantic SEO, RDFa, Linked Data, RDF, Semantic Web, Recommender Systems"@en;
  dc:creator "Martin Hepp"@en;
  owl:versionInfo "V 1.0, Release 2011-10-01"@en;
  dc:rights "The GoodRelations ontology is available under the Creative Commons Attribution 3.0 Unported license; see http://creativecommons.org/licenses/by/3.0/. In a nutshell, you are free to copy, distribute and transmit the work; to remix/adapt the work (e.g. to import the ontology and create specializations of its elements), as long as you attribute the work in the manner specified by the author or licensor (but not in any way that suggests that they endorse you or your use of the work). Proper Attribution: Simply include the statement \"This work is based on the GoodRelations ontology, developed by Martin Hepp\" and link back to http://purl.org/goodrelations/"@en;
  dcterms:license <http://creativecommons.org/licenses/by/3.0/>;
  dc:contributor "Work on the GoodRelations ontology and related research and development has been partly supported by the Austrian BMVIT/FFG under the FIT-IT Semantic Systems project myOntology (grant no. 812515/9284), by a Young Researcher's Grant (Nachwuchsfoerderung 2005-2006) from the Leopold-Franzens-Universitaet Innsbruck, by the European Commission under the project SUPER (FP6-026850), and by the German Federal Ministry of Research (BMBF) by a grant under the KMU Innovativ program as part of the Intelligent Match project (FKZ 01IS10022B). The"@en;
  foaf:homepage <http://purl.org/goodrelations/> .

_:node242 rdf:rest _:node243 .

_:node243 rdf:rest rdf:nil .

gr:isListPrice owl:deprecated true .

gr:Buy owl:deprecated true .

gr:N-Ary-Relations owl:deprecated true .

gr:LocationOfSalesOrServiceProvisioning owl:deprecated true .

gr:ProductOrServicesSomeInstancesPlaceholder owl:deprecated true .

gr:ActualProductOrServiceInstance owl:deprecated true .

gr:PublicHolidays gr:displayPosition 8 .

gr:Wednesday gr:displayPosition 3 .

gr:Thursday gr:displayPosition 4 .

gr:Friday gr:displayPosition 5 .

gr:Tuesday gr:displayPosition 2 .

gr:Monday gr:displayPosition 1 .

gr:Sunday gr:displayPosition 7 .

gr:Saturday gr:displayPosition 6 .

gr:Wednesday gr:hasNext gr:Thursday .

gr:Thursday gr:hasNext gr:Friday .

gr:Friday gr:hasNext gr:Saturday .

gr:Tuesday gr:hasNext gr:Wednesday .

gr:Monday gr:hasNext gr:Tuesday .

gr:Sunday gr:hasNext gr:Monday .

gr:Saturday gr:hasNext gr:Sunday .

gr:Wednesday gr:hasPrevious gr:Tuesday .

gr:Thursday gr:hasPrevious gr:Wednesday .

gr:Friday gr:hasPrevious gr:Thursday .

gr:Tuesday gr:hasPrevious gr:Monday .

gr:Monday gr:hasPrevious gr:Sunday .

gr:Sunday gr:hasPrevious gr:Saturday .

gr:Saturday gr:hasPrevious gr:Friday .

gr:Offering owl:disjointWith gr:BusinessEntity, gr:PriceSpecification, gr:Location,
    gr:BusinessEntityType, gr:TypeAndQuantityNode, gr:OpeningHoursSpecification, gr:ProductOrService,
    gr:DeliveryMethod, gr:PaymentMethod, gr:BusinessFunction, gr:WarrantyPromise, gr:WarrantyScope,
    gr:QuantitativeValue, gr:Brand, gr:DayOfWeek, gr:QualitativeValue .

gr:BusinessEntity owl:disjointWith gr:Offering, gr:PriceSpecification, gr:Location,
    gr:BusinessEntityType, gr:TypeAndQuantityNode, gr:OpeningHoursSpecification, gr:DeliveryMethod,
    gr:PaymentMethod, gr:BusinessFunction, gr:WarrantyPromise, gr:WarrantyScope, gr:QuantitativeValue,
    gr:Brand, gr:DayOfWeek .

gr:PriceSpecification owl:disjointWith gr:Offering, gr:BusinessEntity, gr:Location,
    gr:BusinessEntityType, gr:TypeAndQuantityNode, gr:OpeningHoursSpecification, gr:ProductOrService,
    gr:DeliveryMethod, gr:PaymentMethod, gr:BusinessFunction, gr:WarrantyPromise, gr:WarrantyScope,
    gr:QuantitativeValue, gr:Brand, gr:DayOfWeek .

gr:QuantitativeValueInteger owl:disjointWith gr:QuantitativeValueFloat .

gr:Location owl:disjointWith gr:Offering, gr:BusinessEntity, gr:PriceSpecification,
    gr:BusinessEntityType, gr:TypeAndQuantityNode, gr:OpeningHoursSpecification, gr:DeliveryMethod,
    gr:PaymentMethod, gr:BusinessFunction, gr:WarrantyPromise, gr:WarrantyScope, gr:QuantitativeValue,
    gr:Brand, gr:DayOfWeek .

gr:BusinessEntityType owl:disjointWith gr:Offering, gr:BusinessEntity, gr:PriceSpecification,
    gr:Location, gr:TypeAndQuantityNode, gr:OpeningHoursSpecification, gr:ProductOrService,
    gr:DeliveryMethod, gr:PaymentMethod, gr:BusinessFunction, gr:WarrantyPromise, gr:WarrantyScope,
    gr:QuantitativeValue, gr:Brand, gr:DayOfWeek .

gr:TypeAndQuantityNode owl:disjointWith gr:Offering, gr:BusinessEntity, gr:PriceSpecification,
    gr:Location, gr:BusinessEntityType, gr:OpeningHoursSpecification, gr:ProductOrService,
    gr:DeliveryMethod, gr:PaymentMethod, gr:BusinessFunction, gr:WarrantyPromise, gr:WarrantyScope,
    gr:QuantitativeValue, gr:Brand, gr:DayOfWeek, gr:QualitativeValue .

gr:Individual owl:disjointWith gr:SomeItems, gr:ProductOrServiceModel .

gr:OpeningHoursSpecification owl:disjointWith gr:Offering, gr:BusinessEntity, gr:PriceSpecification,
    gr:Location, gr:BusinessEntityType, gr:TypeAndQuantityNode, gr:ProductOrService, gr:DeliveryMethod,
    gr:PaymentMethod, gr:BusinessFunction, gr:WarrantyPromise, gr:WarrantyScope, gr:QuantitativeValue,
    gr:Brand, gr:DayOfWeek .

gr:ProductOrService owl:disjointWith gr:Offering, gr:PriceSpecification, gr:BusinessEntityType,
    gr:TypeAndQuantityNode, gr:OpeningHoursSpecification, gr:DeliveryMethod, gr:BusinessFunction,
    gr:WarrantyPromise, gr:WarrantyScope, gr:QuantitativeValue, gr:Brand, gr:DayOfWeek .

gr:DeliveryMethod owl:disjointWith gr:Offering, gr:BusinessEntity, gr:PriceSpecification,
    gr:Location, gr:BusinessEntityType, gr:TypeAndQuantityNode, gr:OpeningHoursSpecification,
    gr:ProductOrService, gr:PaymentMethod, gr:BusinessFunction, gr:WarrantyPromise, gr:WarrantyScope,
    gr:QuantitativeValue, gr:Brand, gr:DayOfWeek .

gr:PaymentMethod owl:disjointWith gr:Offering, gr:BusinessEntity, gr:PriceSpecification,
    gr:Location, gr:BusinessEntityType, gr:TypeAndQuantityNode, gr:OpeningHoursSpecification,
    gr:DeliveryMethod, gr:BusinessFunction, gr:WarrantyPromise, gr:WarrantyScope, gr:QuantitativeValue,
    gr:Brand, gr:DayOfWeek .

gr:QuantitativeValueFloat owl:disjointWith gr:QuantitativeValueInteger .

gr:SomeItems owl:disjointWith gr:Individual, gr:ProductOrServiceModel .

gr:BusinessFunction owl:disjointWith gr:Offering, gr:BusinessEntity, gr:PriceSpecification,
    gr:Location, gr:BusinessEntityType, gr:TypeAndQuantityNode, gr:OpeningHoursSpecification,
    gr:ProductOrService, gr:DeliveryMethod, gr:PaymentMethod, gr:WarrantyPromise, gr:WarrantyScope,
    gr:QuantitativeValue, gr:Brand, gr:DayOfWeek .

gr:PaymentChargeSpecification owl:disjointWith gr:DeliveryChargeSpecification, gr:UnitPriceSpecification .

gr:WarrantyPromise owl:disjointWith gr:Offering, gr:BusinessEntity, gr:PriceSpecification,
    gr:Location, gr:BusinessEntityType, gr:TypeAndQuantityNode, gr:OpeningHoursSpecification,
    gr:ProductOrService, gr:DeliveryMethod, gr:PaymentMethod, gr:BusinessFunction, gr:WarrantyScope,
    gr:QuantitativeValue, gr:Brand, gr:DayOfWeek .

gr:ProductOrServiceModel owl:disjointWith gr:BusinessEntity, gr:Individual, gr:SomeItems,
    gr:Brand .

gr:WarrantyScope owl:disjointWith gr:Offering, gr:BusinessEntity, gr:PriceSpecification,
    gr:Location, gr:BusinessEntityType, gr:TypeAndQuantityNode, gr:OpeningHoursSpecification,
    gr:ProductOrService, gr:DeliveryMethod, gr:PaymentMethod, gr:BusinessFunction, gr:WarrantyPromise,
    gr:QuantitativeValue, gr:Brand, gr:DayOfWeek .

gr:QuantitativeValue owl:disjointWith gr:Offering, gr:BusinessEntity, gr:PriceSpecification,
    gr:Location, gr:BusinessEntityType, gr:TypeAndQuantityNode, gr:OpeningHoursSpecification,
    gr:ProductOrService, gr:DeliveryMethod, gr:PaymentMethod, gr:BusinessFunction, gr:WarrantyPromise,
    gr:WarrantyScope, gr:Brand, gr:DayOfWeek, gr:QualitativeValue .

gr:Brand owl:disjointWith gr:Offering, gr:BusinessEntity, gr:PriceSpecification, gr:Location,
    gr:BusinessEntityType, gr:TypeAndQuantityNode, gr:OpeningHoursSpecification, gr:ProductOrService,
    gr:DeliveryMethod, gr:PaymentMethod, gr:BusinessFunction, gr:WarrantyPromise, gr:WarrantyScope,
    gr:QuantitativeValue, gr:DayOfWeek .

gr:DayOfWeek owl:disjointWith gr:Offering, gr:BusinessEntity, gr:PriceSpecification,
    gr:Location, gr:BusinessEntityType, gr:TypeAndQuantityNode, gr:OpeningHoursSpecification,
    gr:ProductOrService, gr:DeliveryMethod, gr:PaymentMethod, gr:BusinessFunction, gr:WarrantyPromise,
    gr:WarrantyScope, gr:QuantitativeValue, gr:Brand .

gr:DeliveryChargeSpecification owl:disjointWith gr:PaymentChargeSpecification, gr:UnitPriceSpecification .

gr:QualitativeValue owl:disjointWith gr:Offering, gr:TypeAndQuantityNode, gr:QuantitativeValue .

gr:UnitPriceSpecification owl:disjointWith gr:PaymentChargeSpecification, gr:DeliveryChargeSpecification .

_:node245 rdf:rest _:node246 .

_:node246 rdf:rest _:node247 .

_:node247 rdf:rest rdf:nil .

_:node249 rdf:rest _:node250 .

_:node250 rdf:rest rdf:nil .

_:node252 rdf:rest _:node253 .

_:node253 rdf:rest rdf:nil .

_:node255 rdf:rest _:node256 .

_:node256 rdf:rest _:node257 .

_:node257 rdf:rest rdf:nil .

_:node259 rdf:rest _:node260 .

_:node260 rdf:rest _:node261 .

_:node261 rdf:rest rdf:nil .

_:node263 rdf:rest _:node264 .

_:node264 rdf:rest _:node265 .

_:node265 rdf:rest rdf:nil .

_:node267 rdf:rest _:node268 .

_:node268 rdf:rest _:node269 .

_:node269 rdf:rest rdf:nil .

_:node271 rdf:rest _:node272 .

_:node272 rdf:rest _:node273 .

_:node273 rdf:rest rdf:nil .

_:node275 rdf:rest _:node276 .

_:node276 rdf:rest rdf:nil .

_:node278 rdf:rest _:node279 .

_:node279 rdf:rest rdf:nil .

_:node281 rdf:rest _:node282 .

_:node282 rdf:rest rdf:nil .

_:node1 owl:hasValue <http://purl.org/procurement/public-contracts-kinds#>;
  owl:onProperty skos:inScheme .

_:node2 owl:hasValue <http://purl.org/procurement/public-contracts-procedure-types#>;
  owl:onProperty skos:inScheme .

_:node6 owl:hasValue <http://purl.org/procurement/public-contracts-authority-kinds#>;
  owl:onProperty skos:inScheme .

_:node7 owl:hasValue <http://purl.org/procurement/public-contracts-activities#>;
  owl:onProperty skos:inScheme .

_:node3 owl:unionOf _:node4 .

_:node8 owl:unionOf _:node9 .

_:node11 owl:unionOf _:node12 .

_:node14 owl:unionOf _:node15 .

_:node18 owl:unionOf _:node19 .

_:node22 owl:unionOf _:node23 .

_:node26 owl:unionOf _:node27 .

_:node31 owl:unionOf _:node32 .

_:node34 owl:unionOf _:node35 .

_:node37 owl:unionOf _:node38 .

_:node41 owl:unionOf _:node42 .

_:node45 owl:unionOf _:node46 .

_:node54 owl:unionOf _:node55 .

_:node57 owl:unionOf _:node58 .

_:node60 owl:unionOf _:node61 .

_:node63 owl:unionOf _:node64 .

_:node67 owl:unionOf _:node68 .

_:node70 owl:unionOf _:node71 .

_:node73 owl:unionOf _:node74 .

_:node79 owl:unionOf _:node80 .

_:node82 owl:unionOf _:node83 .

_:node85 owl:unionOf _:node86 .

_:node89 owl:unionOf _:node90 .

_:node94 owl:unionOf _:node95 .

_:node98 owl:unionOf _:node99 .

_:node101 owl:unionOf _:node102 .

_:node104 owl:unionOf _:node105 .

_:node107 owl:unionOf _:node108 .

_:node110 owl:unionOf _:node111 .

_:node139 owl:unionOf _:node140 .

_:node142 owl:unionOf _:node143 .

_:node145 owl:unionOf _:node146 .

_:node148 owl:unionOf _:node149 .

_:node151 owl:unionOf _:node152 .

_:node154 owl:unionOf _:node155 .

_:node157 owl:unionOf _:node158 .

_:node162 owl:unionOf _:node163 .

_:node166 owl:unionOf _:node167 .

_:node169 owl:unionOf _:node170 .

_:node174 owl:unionOf _:node175 .

_:node179 owl:unionOf _:node180 .

_:node182 owl:unionOf _:node183 .

_:node185 owl:unionOf _:node186 .

_:node191 owl:unionOf _:node192 .

_:node220 owl:unionOf _:node221 .

_:node223 owl:unionOf _:node224 .

_:node227 owl:unionOf _:node228 .

_:node231 owl:unionOf _:node232 .

_:node234 owl:unionOf _:node235 .

_:node238 owl:unionOf _:node239 .

_:node241 owl:unionOf _:node242 .

_:node244 owl:unionOf _:node245 .

_:node248 owl:unionOf _:node249 .

_:node251 owl:unionOf _:node252 .

_:node254 owl:unionOf _:node255 .

_:node258 owl:unionOf _:node259 .

_:node262 owl:unionOf _:node263 .

_:node266 owl:unionOf _:node267 .

_:node270 owl:unionOf _:node271 .

_:node274 owl:unionOf _:node275 .

_:node277 owl:unionOf _:node278 .

_:node280 owl:unionOf _:node281 .

_:node165 gr:category "42";
  gr:description "VGhlIFNldmVuIE5vYWhpZGUgTGF3cw0KMS4gQmVsaWVmIGluIEctZA0KMi4gUmVzcGVjdCBHLWQgYW5kIHByYWlzZSBoaW0NCjMuIFJlc3BlY3QgaHVtYW4gbGlmZQ0KNC4gUmVzcGVjdCB0aGUgZmFtaWx5DQo1LiBSZXNwZWN0IGh1bWFuIGJlaW5ncw0KNi4gSGF2ZSBhIGp1ZGljaWFsIHN5c3RlbQ0KNy4gUmVzcGVjdCBhbGwgY3JlYXR1cmVz" .
